extraction/Interop.ml
@@ -1,4 +1,0 @@
-module Ocaml_Map_Int = Map.Make(Int)
-module Ocaml_Set_Int = Set.Make(Int)
-
-let remove_all m s = Ocaml_Set_Int.fold Ocaml_Map_Int.remove s m
