MECMAR/props/Correctness.v
@@ -1,5 +1,5 @@
 From Coq Require Import PeanoNat ZArith Bool Lia Program.Equality.
-From Warblre Require Import Tactics Specialize Focus Result Base Patterns StaticSemantics Notation Semantics Definitions.
+From Warblre Require Import List Tactics Specialize Focus Result Base Patterns StaticSemantics Notation Semantics Definitions.
 
 Import Result.Notations.
 Import Semantics.
@@ -8,8 +8,6 @@ Module Correctness.
   Import Patterns.
   Import Notation.
   Import Semantics.
-
-  Notation "'fsuccess' x" := (Success (Some x)) (at level 50, only parsing).
 
   Create HintDb Warblre.
   #[export] Hint Unfold repeatMatcherFuel wrap_option : Warblre.
@@ -21,12 +19,78 @@ Module Correctness.
   #[export]
   Hint Rewrite -> is_not_failure_true_rewrite is_not_failure_false_rewrite : Warblre.
 
+  Ltac clean := repeat
+  (   autounfold with Warblre_coercions in *
+  ||  lazymatch goal with
+      | [ Eq: Success _ = Success _ |-_] => injection Eq as Eq
+      end).
+
+
   (** Progress: We say that a MatchState (wrapped in Result) ry has progressed w.r.t to another MatchState x if:
       - ry = Success y, x and y share the same input string and either
         + direction is forward, in which case x's endIndex <= y's endIndex
         + direction is backward, in which case y's endIndex <= x's endIndex
       - ry is any kind of failure
   *)
+
+  Module Captures.
+    Definition Valid (rer: RegExp) (ls: list nat) := List.Forall.Forall ls (fun i => i < RegExp.capturingGroupsCount rer).
+    
+(*     Lemma combine: forall rer ls ls', Valid rer ls -> Valid rer ls' -> Valid rer (ls ++ ls'). *)
+  End Captures.
+
+  Module Groups.
+    Inductive Bounded: Regex -> nat -> Prop :=
+    | gbEmpty: forall n, Bounded Empty n
+    | gbChar: forall c n, Bounded (Char c) n
+    | gbDisjunction: forall r1 r2 n, Bounded r1 n -> Bounded r2 n -> Bounded (Disjunction r1 r2) n
+    | gbQuantified: forall r q n, Bounded r n -> Bounded (Quantified r q) n
+    | gbSeq: forall r1 r2 n, Bounded r1 n -> Bounded r2 n -> Bounded (Seq r1 r2) n
+    | gbGroup: forall r id n, (id < n)%nat -> Bounded r n -> Bounded (Group id r) n
+    (* Assertions: ^ $ \b \B *)
+    | gbLookahead: forall r n, Bounded r n -> Bounded (Lookahead r) n
+    | gbNegativeLookahead: forall r n, Bounded r n -> Bounded (NegativeLookahead r) n
+    | gbLookback: forall r n, Bounded r n -> Bounded (Lookback r) n
+    | gbNegativeLookbehind: forall r n, Bounded r n -> Bounded (NegativeLookbehind r) n
+    | gbBackReference: forall id n, (id < n)%nat -> Bounded (BackReference id) n.
+
+    Lemma monotony: forall r n n',
+      (n <= n')%nat -> Bounded r n -> Bounded r n'.
+    Proof.
+      intros.
+      induction r;
+        match goal with | [ H: Bounded ?r _ |- _ ] => is_compound r; dependent destruction H end;
+        constructor; fforward; solve [ assumption | lia ].
+    Qed.
+
+    Local Ltac maxify n m eq :=
+      let x := fresh "n" in let Tmp1 := fresh "TMP" in let Tmp2 := fresh "TMP" in
+      remember (Nat.max n m) as x eqn:eq;
+      assert (n <= x) as Tmp1 by lia;
+      assert (m <= x) as Tmp2 by lia;
+      repeat lazymatch goal with
+        | [ H: Bounded ?r n |-_] => pose proof (monotony _ _ _ Tmp1 H); clear H
+        | [ H: Bounded ?r m |-_] => pose proof (monotony _ _ _ Tmp2 H); clear H
+      end;
+      clear Tmp1 Tmp2.
+
+    Lemma existence: forall r, exists n, Bounded r n.
+    Proof.
+      induction r; repeat (maxify + lazymatch goal with
+        | [ H: exists n, Bounded _ n |-_] => destruct H as [ ?n H ]
+        | [ n: nat, m: nat |-_] => let Tmp := fresh "TMP" in maxify n m Tmp; clear n m Tmp
+        | [ n: nat |- exists _, _ ] => solve [ exists n; constructor; assumption ]
+        | [ |- exists _, _ ] => solve [ exists 0; constructor; assumption ]
+        end).
+      - maxify n id Eq_n0. exists (n0 + 1). constructor; try lia. apply monotony with (2 := H). lia.
+      - exists (id + 1). constructor. lia.
+    Qed.
+
+    Lemma capturesWithinValid: forall r rer,
+      Bounded r (RegExp.capturingGroupsCount rer) -> Captures.Valid rer (capturingGroupsWithin r).
+    Proof.
+    Admitted.
+  End Groups.
 
   (* Allows to abstract most theorem over the direction of progress *)
   Inductive directionalProgress: direction -> MatchState -> MatchState -> Prop :=
@@ -37,27 +101,102 @@ Module Correctness.
   | pStep: forall dir x y, 
       (MatchState.input x) = (MatchState.input y)
     -> directionalProgress dir x y
-    -> progress dir x (fsuccess y)
+    -> progress dir x (Success (Some y))
   | pMismatch: forall dir x, progress dir x failure
   | pError: forall dir x f, progress dir x (Failure f).
   #[export]
   Hint Constructors progress: core.
 
-  Definition OnInput (x: MatchState) (str: list Character) := MatchState.input x = str.
-  Definition Valid (x: MatchState) := (0 <= MatchState.endIndex x <= Z.of_nat (length (MatchState.input x)))%Z.
+  Definition IteratorOn (str: list Character) (i: Z) := (0 <= i <= Z.of_nat (length str))%Z.
+
+  Module CaptureRange.
+    Inductive Valid (str: list Character): option CaptureRange -> Prop :=
+    | vCrDefined: forall s e, ( s <= e -> IteratorOn str s -> IteratorOn str e -> Valid str (Some (capture_range s e)) )%Z
+    | vCrUndefined: Valid str undefined.
+
+    Ltac normalize := repeat
+    (   cbn
+    ||  autounfold with Warblre_coercions in *
+    ||  unfold IteratorOn in *
+    ||  match goal with
+        | [ Eq: Success (capture_range _ _ _) = Success ?s |-_] => injection Eq as <-
+        | [ Eq: Success ?s = Success (capture_range _ _ _) |-_] => injection Eq as ->
+        | [ c: CaptureRange |- _ ] => let s := fresh c "_start" in
+                                      let e := fresh c "_end" in
+                                      destruct c as [ s e ]
+        | [ VCs : List.Forall.Forall ?c (CaptureRange.Valid ?str),
+            Indexed : (?c [?n]) = Success (Some (capture_range ?s ?e))
+          |- _ ] => is_var c; lazymatch goal with
+                    | [ _: (s <= e)%Z |- _ ] => fail
+                    | [ |- _ ] => let H := fresh "VCR_" s "_" e in
+                                  pose proof (VCs _ _ Indexed) as H;
+                                  dependent destruction H
+                    end
+        | [ VC: CaptureRange.Valid _ (Some (capture_range ?s ?e)) |- _ ] =>
+            dependent destruction VC
+        | [ |- CaptureRange.Valid _ _ ] => constructor
+        | [ Eq: _ = _ |- _ ] => match type of Eq with
+          | Success ?x = Success _ =>
+            (check_type x CaptureRange + check_type x (option CaptureRange));
+            injection Eq; clear Eq; intros Eq
+          | ?s = ?x =>
+            is_var s;
+            (check_type x CaptureRange + check_type x (option CaptureRange) + check_type x (Result (option CaptureRange) MatchError));
+            subst s
+          | ?x = ?s =>
+            is_var s;
+            (check_type x CaptureRange + check_type x (option CaptureRange) + check_type x (Result (option CaptureRange) MatchError));
+            subst s
+          end
+        end).
+
+    Ltac solvers t := lazymatch goal with
+    | [ Eq: List.Update.Nat.One.update (Some (capture_range ?s ?e)) ?c _ = Success ?c',
+        H: List.Forall.Forall ?c (CaptureRange.Valid ?str)
+        |- List.Forall.Forall ?c' _ ] =>
+          refine (List.Update.Nat.One.prop_preservation _ _ _ _ _ H _ Eq); constructor; unfold IteratorOn; t
+    | [ H: List.Forall.Forall ?oc (CaptureRange.Valid ?str),
+        Eq: List.Update.Nat.Batch.update _ ?oc _ = Success ?nc
+      |- List.Forall.Forall ?nc (CaptureRange.Valid ?str) ] =>
+          refine (List.Update.Nat.Batch.prop_preservation _ _ _ _ _ H _ Eq); solve [ constructor | assumption | t ]
+    end.
+
+    Local Ltac solve_impl t := solve [ normalize; (solvers || t) ].
+
+    Ltac solve := solve_impl idtac.
+    Ltac solve_with t := solve_impl t.
+  End CaptureRange.
 
   Module MatchState.
-    Lemma characterClass_successful_state_Valid: forall input endIndex captures dir,
+    (* Lemma characterClass_successful_state_Valid: forall input endIndex captures dir,
       ~ (step{dir} endIndex < 0)%Z  ->
       ~ (Z.of_nat (length input) < step{dir} endIndex)%Z ->
-      Valid (Definitions.characterClass_successful_state input endIndex captures dir).
-    Proof. destruct dir; constructor; cbn in *; lia. Qed.
+      Valid input (Definitions.characterClass_successful_state input endIndex captures dir).
+    Proof. destruct dir; constructor; cbn in *; lia. Qed. *)
 
+    Definition OnInput (str: list Character) (x: MatchState) := MatchState.input x = str.
+    Definition Valid (str: list Character) (rer: RegExp) (x: MatchState) :=
+      OnInput str x /\
+      IteratorOn str (MatchState.endIndex x) /\
+      length (MatchState.captures x) = RegExp.capturingGroupsCount rer /\
+      List.Forall.Forall (MatchState.captures x) (CaptureRange.Valid str).
+
+    Lemma change_captures: forall str rer input endIndex cap cap',
+      length cap' = RegExp.capturingGroupsCount rer ->
+      List.Forall.Forall cap' (CaptureRange.Valid str) ->
+      Valid str rer (match_state input endIndex cap) ->
+      Valid str rer (match_state input endIndex cap').
+    Proof.
+      intros str rer input endIndex cap cap' H0 H1 [ OI_x [ IO_x V_cap ]]. 
+      unfold Valid. split_conjs; try assumption.
+    Qed.
+    
     (*  Normalizes all MatchStates by doing the following:
         - Destructing them into their components
         - Then, if the MatchState is known to be on a particular string, eliminate the string introduced at the previous step. *)
     Ltac normalize := repeat
-    (   simpl (match_state _ _ _) in *
+    (   CaptureRange.normalize
+    ||  simpl (match_state _ _ _) in *
     ||  simpl (MatchState.input _) in *
     ||  simpl (MatchState.endIndex _) in *
     ||  simpl (MatchState.captures _) in *
@@ -82,20 +221,48 @@ Module Correctness.
           let endIndex := fresh "endIndex_" x in
           let captures := fresh "captures_" x in
           destruct x as [ input endIndex captures ]
-        | [ H: OnInput (match_state ?input _ _) ?str |- _ ] =>
+        | [ H: OnInput ?str (match_state ?input _ _) |- _ ] =>
           unfold OnInput in H; cbn in H;
           try rewrite -> H in *; clear H; clear input
+        | [ H: MatchState.Valid ?str _ (match_state ?input ?endIndex ?captures) |- _ ] =>
+          let OI := fresh "Eq_" input in
+          let Iterx := fresh "Iter_" endIndex in
+          let VCL := fresh "VCL_" captures in
+          let VCF := fresh "VCF_" captures in
+          let Tmp := fresh "TMP" in
+          destruct H as [ OI [ Iterx [ VCL VCF ]]];
+          try rewrite -> Tmp in *
+        | [ |- MatchState.Valid _ _ _ ] =>
+          unfold Valid; split_conjs
+
+        | [ H: List.Update.Nat.One.update _ _ _ = Success _ |- _ ] =>
+          pose proof (List.Update.Nat.One.success_length _ _ _ _ H) as <-
+        | [ H: List.Update.Nat.Batch.update _ _ _ = Success _ |- _ ] =>
+          pose proof (List.Update.Nat.Batch.success_length _ _ _ _ H) as <-
         end).
 
-    Local Ltac solvers := assumption || reflexivity || (Zhelper; apply characterClass_successful_state_Valid; assumption).
+    Ltac solvers t := assumption || reflexivity || CaptureRange.solvers t (*|| (Zhelper; apply characterClass_successful_state_Valid; assumption)*).
     (* Solves the current goal by 1. normalizing the states 2. leveraging assumptions and reflexivity *)
-    Ltac solve := normalize; solve [ solvers ].
+    Local Ltac solve_impl t := solve [ normalize; unfold OnInput, Valid; (solvers t || t) ].
+
+    Ltac solve := solve_impl idtac.
+    Ltac solve_with t := solve_impl t.
+
+
+    Definition init (rer: RegExp) (str: list Character) (i: nat) := (match_state str (Z.of_nat i) (List.repeat None (RegExp.capturingGroupsCount rer))).
+
+    Lemma valid_init: forall rer str i, (i <= length str) -> Valid str rer (init rer str i).
+    Proof.
+      intros rer str i Ineq_i. normalize; try MatchState.solve_with lia.
+      - apply List.repeat_length.
+      - apply List.Forall.repeat. constructor.
+    Qed.
   End MatchState.
 
   Module Progress.
     Local Ltac hammer :=
       repeat match goal with
-      | [ H: progress _ _ (fsuccess _) |- _ ] => inversion H; clear H; subst
+      | [ H: progress _ _ (Success (Some _)) |- _ ] => inversion H; clear H; subst
       | [ H: directionalProgress ?d _ _ |- _ ] => is_constructor d; inversion H; clear H
       | [ _: directionalProgress ?d _ _ |- _ ] => destruct d
       | [ |- progress _ _ ?y ] => is_var y; let Eq := fresh "Eq" y in destruct y eqn:Eq
@@ -106,18 +273,18 @@ Module Correctness.
       | [ |- directionalProgress ?d _ _ ] => destruct d
       end.
 
-    Lemma step: forall x dir, progress dir x (fsuccess (match_state 
+    Lemma step: forall x dir n, (0 <= n)%Z -> progress dir x (Success (Some (match_state 
         (MatchState.input x)
         (if Direction.eqb dir forward
-         then (MatchState.endIndex x + 1)%Z
-         else (MatchState.endIndex x - 1)%Z) 
-        (MatchState.captures x))).
+         then (MatchState.endIndex x + n)%Z
+         else (MatchState.endIndex x - n)%Z) 
+        (MatchState.captures x)))).
     Proof. intros. destruct dir; (constructor; cbn in *; solve [ assumption | constructor; cbn; lia ]). Qed.
 
-    Lemma refl: forall dir x, (progress dir) x (fsuccess x).
+    Lemma refl: forall dir x, (progress dir) x (Success (Some x)).
     Proof. intros. hammer. 1,3: congruence. all: lia. Qed.
 
-    Lemma trans: forall dir x y z, (progress dir) x (fsuccess y) -> (progress dir) y z -> (progress dir) x z.
+    Lemma trans: forall dir x y z, (progress dir) x (Success (Some y)) -> (progress dir) y z -> (progress dir) x z.
     Proof.
       intros. hammer.
       1,3: congruence.
@@ -125,8 +292,8 @@ Module Correctness.
     Qed.
 
     Lemma ignores_captures_r: forall c1 c2 dir x i n,
-          (progress dir) x (fsuccess (i [@ n $ c1]))
-      <-> (progress dir) x (fsuccess (i [@ n $ c2])).
+          (progress dir) x (Success (Some (i [@ n $ c1])))
+      <-> (progress dir) x (Success (Some (i [@ n $ c2]))).
     Proof.
       intros; split; intros; hammer; subst.
       all: try assumption.
@@ -142,7 +309,7 @@ Module Correctness.
       all: cbn in *; lia.
     Qed.
 
-    Lemma progress_same_input: forall dir x y, progress dir x (fsuccess y)
+    Lemma progress_same_input: forall dir x y, progress dir x (Success (Some y))
       -> MatchState.input x = MatchState.input y.
     Proof. intros. inversion H. assumption. Qed.
 
@@ -152,11 +319,11 @@ Module Correctness.
         - Derives that two MatchStates have the same input from progress hypotheses *)
     Ltac normalize := repeat (
         MatchState.normalize
-    ||  rewrite <- (ignores_captures_l (DMap.empty _)) in *
-    ||  rewrite <- (ignores_captures_r (DMap.empty _)) in *
+    ||  rewrite <- (ignores_captures_l (List.empty)) in *
+    ||  rewrite <- (ignores_captures_r (List.empty)) in *
     ||  lazymatch goal with
-        | [ H: progress _ (?i [@ _ $ _]) (fsuccess (?i [@ _ $ _])) |- _ ] => fail
-        | [ H: progress _ (?i1 [@ _ $ _]) (fsuccess (?i2 [@ _ $ _])) |- _ ] =>
+        | [ H: progress _ (?i [@ _ $ _]) (Success (Some (?i [@ _ $ _]))) |- _ ] => fail
+        | [ H: progress _ (?i1 [@ _ $ _]) (Success (Some (?i2 [@ _ $ _]))) |- _ ] =>
           let Tmp := fresh in
           pose proof progress_same_input as Tmp;
           specialize Tmp with (1 := H);
@@ -168,10 +335,10 @@ Module Correctness.
 
     Local Ltac solvers := assumption || apply step || apply refl || reflexivity || MatchState.solve.
     (* Solves the current goal by 1. normalizing progress 2. leveraging assumptions and reflexivity *)
-    Ltac solve := normalize; solve [ solvers ].
+    Ltac solve := solve [ normalize; solvers ].
 
     Ltac saturate_step := normalize; match goal with
-    | [ H1: progress ?dir ?x (fsuccess ?y), H2: progress ?dir ?y (Success ?z) |- _ ] =>
+    | [ H1: progress ?dir ?x (Success (Some ?y)), H2: progress ?dir ?y (Success ?z) |- _ ] =>
       let H := fresh "ps_trans_" H1 H2 in
       pose proof Progress.trans as H;
       specialize H with (1 := H1) (2 := H2);
@@ -185,195 +352,420 @@ Module Correctness.
   (** Intermediate value: We say that Matcher _honores its continuation_ if 
       its continuation must succeed on an input the matcher called it with in order for the matcher to itself succeed. *)
   Module IntermediateValue.
-    (* y is also most likely Valid; see if we can incorporate this to the definition *)
-    Definition HonoresContinuation (m: Matcher) (dir: direction) := forall x c z, m x c = fsuccess z -> exists y, progress dir x (fsuccess y) /\ c y = fsuccess z.
+    Definition HonoresContinuation (str: list Character) (rer: RegExp) (m: Matcher) (dir: direction) := forall x c z,
+      (* For any valid state *)
+      MatchState.Valid str rer x ->
+      (* If the overall computation succeeded *)
+      m x c = Success (Some z) ->
+      (* There is an intermediate value y that was produced by m and then passed to c which then succeeded. *)
+      exists y, MatchState.Valid str rer y /\ progress dir x (Success (Some y)) /\ c y = Success (Some z).
     #[export]
     Hint Unfold HonoresContinuation : Warblre.
 
-    Ltac search := subst; lazymatch goal with
+    (*  Automated tactic to find the intermediate value 
+        It will also try to prove the conditions on the intermediate value.
+      *)
+    Ltac search := autounfold with Warblre_coercions in *; subst; lazymatch goal with
     | [ H: Success _ = Success _ |- _ ] => injection H; clear H; intros H; search
-    | [ H: ?c ?y = Success ?z |- exists x, progress ?dir _ _ /\ ?c x = Success ?z ] =>
-      exists y; split;
-      [ try solve [Progress.saturate]
+    | [ H: ?c ?y = Success ?z |- exists x, MatchState.Valid _ _ _ /\ progress ?dir _ _ /\ ?c x = Success ?z ] =>
+      exists y; split_conjs;
+      [ assumption + ( unfold MatchState.Valid; split_conjs; try MatchState.solve )
+      | try solve [Progress.saturate]
       | apply H ]
     end.
 
-    Lemma repeatMatcher: forall fuel dir m min max greedy groupsWithin,
-          HonoresContinuation m dir -> HonoresContinuation (fun x c => repeatMatcher' m min max greedy x c groupsWithin fuel) dir.
+    (** TODO: move to Tactics.v *)
+    Ltac fforward_impl H0 By := lazymatch type of H0 with
+    | (?x = ?x) -> ?Q => specialize (H0 (eq_refl x))
+    | ?P -> ?Q => lazymatch goal with
+      | [ H1: P |- _ ] => specialize (H0 H1); fforward_impl H0 By
+      | [ |- _ ] => let Tmp := fresh "Tmp" in assert (P) as Tmp; [ try solve[By] | specialize (H0 Tmp); clear Tmp; fforward_impl H0 By ]
+      end
+    | _ => idtac
+    end.
+
+    Tactic Notation "fforward" hyp(H) := fforward_impl H idtac.
+    Tactic Notation "fforward" hyp(H) "as" simple_intropattern(I) := fforward_impl H idtac; destruct H as I.
+    Tactic Notation "fforward" hyp(H) "by" tactic(t) := fforward_impl H t.
+    Tactic Notation "fforward" hyp(H) "as" simple_intropattern(I) "by" tactic(t) := fforward_impl H t; destruct H as I.
+    (** End TODO *)
+
+    Lemma repeatMatcher: forall str rer fuel dir m min max greedy groupsWithin,
+          HonoresContinuation str rer m dir ->
+          HonoresContinuation str rer (fun x c => repeatMatcher' m min max greedy x c groupsWithin fuel) dir.
     Proof.
+      (* The 'recursive' case (i.e. when min is not zero or the endIndex is different from last iteration) *)
+      assert (forall x z s c str rer fuel dir m min max greedy groups,
+        MatchState.Valid str rer x ->
+        List.Update.Nat.Batch.update None (MatchState.captures x) groups = Success s ->
+        HonoresContinuation str rer m dir ->
+        (forall dir m min max greedy groups,
+          HonoresContinuation str rer m dir ->
+          HonoresContinuation str rer (Definitions.RepeatMatcher.matcher m min max greedy groups fuel) dir) ->
+        (m (match_state (MatchState.input x) (MatchState.endIndex x) s)
+          (Definitions.RepeatMatcher.continuation x c m min max greedy groups fuel) = Success (Some z)) ->
+        exists y : MatchState,
+          MatchState.Valid str rer y /\ progress dir x (Success (Some y)) /\ c y = Success (Some z)
+      ) as Rec. {
+        intros x z s c str rer fuel dir m min max greedy groups Vx Ex_s HCm IH Eq_rec.
+        unfold HonoresContinuation in HCm, IH.
+        specialize IH with (1 := HCm).
+        focus § _ (_ _ []) _ § remember as d in Eq_rec.
+        specialize HCm with (2 := Eq_rec).
+        fforward HCm as [ y0 [ Vy0 [ Pxy0 Eq_dy0 ]] ] by MatchState.solve.
+        rewrite -> Heqd in Eq_dy0. unfold Definitions.RepeatMatcher.continuation in Eq_dy0.
+        focus § _ [] _ § auto destruct in Eq_dy0.
+        specialize IH with (2 := Eq_dy0). fforward IH as [ y1 [ Vy1 [ Py0y1 Eq_cy1 ]]].
+        search.
+      }
+
       induction fuel; [ discriminate | ].
-      deltaf repeatMatcher'. cbn. intros dir m min max greedy groupsWithin HCm x c z H.
-      focus § _ [] _ § auto destruct in H; autounfold with Warblre in *.
-      - IntermediateValue.search.
-      - auto_specialize; Coq.Program.Tactics.destruct_conjs.
-        focus § _ [] _ § auto destruct in H3.
-        auto_specialize; Coq.Program.Tactics.destruct_conjs.
-        IntermediateValue.search.
-      - IntermediateValue.search.
-      - auto_specialize; Coq.Program.Tactics.destruct_conjs.
-        focus § _ [] _ § auto destruct in H3.
-        auto_specialize; Coq.Program.Tactics.destruct_conjs.
-        IntermediateValue.search.
-      - bookkeeper. auto_specialize; Coq.Program.Tactics.destruct_conjs.
-        focus § _ [] _ § auto destruct in H2.
-        auto_specialize; Coq.Program.Tactics.destruct_conjs.
-        IntermediateValue.search.
-      - IntermediateValue.search.
+      cbn. intros dir m min max greedy groupsWithin HCm x c z Vx H.
+      focus § _ [] _ § auto destruct in H.
+      - search.
+      - eapply Rec; eassumption.
+      - search.
+      - eapply Rec; eassumption.
+      - injection H as [=->].
+        eapply Rec; eassumption.
+      - search.
     Qed.
 
-    Lemma compileSubPattern: forall r rer dir, HonoresContinuation (compileSubPattern r rer dir) dir.
+    Lemma characterSetMatcher: forall str rer A invert dir,
+          HonoresContinuation str rer (characterSetMatcher rer A invert dir) dir.
     Proof.
-      induction r; intros rer dir x c z; cbn;
+      intros str rer A invert dir x c z Vx Eq_z.
+      unfold characterSetMatcher in Eq_z. focus § _ [] _ § auto destruct in Eq_z.
+      search.
+      - Zhelper. MatchState.normalize. lia.
+      - apply Progress.step. lia.
+    Qed.
+
+    Lemma backreferenceMatcher: forall str rer n dir,
+          HonoresContinuation str rer (backreferenceMatcher rer n dir) dir.
+    Proof.
+      unfold HonoresContinuation. intros str rer n dir x c z Vx Eq_z.
+      unfold backreferenceMatcher in Eq_z. focus § _ [] _ § auto destruct in Eq_z.
+      - search.
+      - search.
+        + destruct dir; MatchState.normalize; cbn in *; lia.
+        + apply Progress.step. MatchState.normalize. cbn in *. lia.
+    Qed.
+
+    Lemma compileSubPattern: forall r str rer dir,
+      HonoresContinuation str rer (compileSubPattern r rer dir) dir.
+    Proof.
+      induction r; intros str rer dir x c z; cbn;
       focus § _ [] _ -> _ § auto destruct.
-      + intros. IntermediateValue.search.
-      + intros. IntermediateValue.search.
-      + intros. bookkeeper. autounfold with Warblre in *. repeat (specialize_once; Coq.Program.Tactics.destruct_conjs). IntermediateValue.search.
-      + intros. bookkeeper. autounfold with Warblre in *. repeat (specialize_once; Coq.Program.Tactics.destruct_conjs). IntermediateValue.search.
-      + apply IntermediateValue.repeatMatcher. apply IHr.
-      + intros. bookkeeper. autounfold with Warblre in *. repeat (specialize_once; Coq.Program.Tactics.destruct_conjs). IntermediateValue.search.
-      + intros. bookkeeper. autounfold with Warblre in *. repeat (specialize_once; Coq.Program.Tactics.destruct_conjs). IntermediateValue.search.
-      + intros. bookkeeper. autounfold with Warblre in *. repeat (specialize_once; Coq.Program.Tactics.destruct_conjs).
-        focus §_ [] _§ auto destruct in H1. IntermediateValue.search.
-      + intros. IntermediateValue.search.
-      + intros. IntermediateValue.search.
-      + intros. IntermediateValue.search.
-      + intros. IntermediateValue.search.
+      - intros; search.
+      - apply characterSetMatcher.
+      - intros Vx Eq_z.
+        autounfold with Warblre in *.
+        focus § _ [] _ § auto destruct in Eq_z.
+        + injection Eq_z as ->. apply IHr1 with (2 := AutoDest_). apply Vx.
+        + apply IHr2 with (2 := Eq_z). apply Vx.
+      - apply repeatMatcher. apply IHr.
+      - intros Vx Eq_z.
+        autounfold with Warblre in *.
+        focus § _ [] _ § auto destruct in Eq_z.
+        + specialize IHr1 with (1 := Vx) (2 := Eq_z) as [y0 [Vy0 [Pxy0 Eq_y0]]].
+          specialize IHr2 with (1 := Vy0) (2 := Eq_y0) as [y1 [Vy1 [Pxy1 Eq_y1]]].
+          search.
+        + specialize IHr2 with (1 := Vx) (2 := Eq_z) as [y0 [Vy0 [Pxy0 Eq_y0]]].
+          specialize IHr1 with (1 := Vy0) (2 := Eq_y0) as [y1 [Vy1 [Pxy1 Eq_y1]]].
+          search.
+      - intros Vx Eq_z.
+        autounfold with Warblre in *.
+        specialize IHr with (str := str) (1 := Vx) (2 := Eq_z) as [y [Vy [Pxy Eq_y]]].
+        focus § _ [] _ § auto destruct in Eq_y.
+        search.
+        MatchState.normalize.
+        refine (List.Update.Nat.One.prop_preservation _ _ _ _ _ VCF_captures_y _ AutoDest_0).
+        focus § _ [] _ § auto destruct in AutoDest_; injection AutoDest_ as <-; Zhelper; MatchState.normalize; lia.
+      - intros Vx Eq_z.
+        autounfold with Warblre in *.
+        focus § _ [] _ § auto destruct in Eq_z.
+        specialize IHr with (1 := Vx) (2 := AutoDest_) as [y [Vy [Pxy Eq_y]]].
+        search.
+      - intros Vx Eq_z.
+        autounfold with Warblre in *.
+        focus § _ [] _ § auto destruct in Eq_z.
+        search.
+      - intros Vx Eq_z.
+        autounfold with Warblre in *.
+        focus § _ [] _ § auto destruct in Eq_z.
+        specialize IHr with (1 := Vx) (2 := AutoDest_) as [y [Vy [Pxy Eq_y]]].
+        search.
+      - intros Vx Eq_z.
+        autounfold with Warblre in *.
+        focus § _ [] _ § auto destruct in Eq_z.
+        search.
+      - apply backreferenceMatcher.
     Qed.
   End IntermediateValue.
 
-  (** Monotony: We say that Matcher(Continuation) is
-    + A _Forward_ Matcher(Continuation) if for any input (x: MatchState), the then returned (y: MatchState) is a foward progress;
-    + A _Backward_ Matcher(Continuation) if for any input (x: MatchState), the then returned (y: MatchState) is a backward progress;
-    + A _Stationary_ Matcher(Continuation) if it is both a Forward and Backward Matcher(Continuation). *)
   Module Monotony.
-    Definition MonotonousContinuation (dir: direction) (c: MatcherContinuation) :=
-      forall x, (progress dir) x (c x).
-    Definition MonotonousMatcher (dir: direction) (m: Matcher) :=
-      forall x c,
-          MonotonousContinuation dir c
-      ->  progress dir x (m x c).
-    #[export]
-    Hint Unfold MonotonousContinuation MonotonousMatcher : Warblre.
-
-    Lemma compileSubPattern: forall r rer dir, MonotonousMatcher dir (compileSubPattern r rer dir).
+    Lemma compilePattern: forall r rer input i,
+      progress forward (match_state input (Z.of_nat i) (List.repeat None (RegExp.capturingGroupsCount rer))) (compilePattern r rer input i).
     Proof.
-      intros r rer dir x c Mc.
-      (focus § _ _ _ []§ do (fun t => destruct t as [ [ s | ] | ] eqn:Suc)); try easy.
-      apply IntermediateValue.compileSubPattern with (dir := dir) in Suc.
-      destruct Suc as [ y [ Pxy Suc ] ]. rewrite <- Suc.
-      apply Progress.trans with (y := y).
-      + assumption.
-      + apply Mc.
-    Qed.
-
-    Lemma compilePattern: forall r rer input i, progress forward (match_state input (Z.of_nat i) (DMap.empty (option  CaptureRange))) (compilePattern r rer input i).
-    Proof.
-      intros. delta compilePattern. cbn.
-      focus § _ _ _ [] § auto destruct.
+      intros r rer input i.
+      delta compilePattern.
+      cbn. focus § _ _ _ [] § auto destruct.
       - constructor.
-      - apply compileSubPattern.
-        intros x. apply Progress.refl.
+      - boolean_simplifier. spec_reflector PeanoNat.Nat.leb_spec0.
+        (* Assert that the start state is valid *)
+        focus § _ _ [] _ § do (fun x => assert (MatchState.Valid input rer x) as V_x). {
+          constructor.
+          + subst. MatchState.solve.
+          + subst. split_conjs.
+            * subst. cbn. constructor; lia.
+            * cbn. rewrite -> List.repeat_length. reflexivity.
+            * intros j v Indexed.
+              cbn in Indexed. apply List.Indexing.Nat.repeat in Indexed. subst.
+              constructor.
+        }
+        (* Eval program; most cases are trivial since they fail *)
+        (focus § _ _ _ [] § do (fun t => destruct t as [ [ z | ] | ] eqn:Eq_z)); try solve[ constructor ].
+        (* Use the intermediate value lemma to conclude *)
+        pose proof (IntermediateValue.compileSubPattern _ _ _ _ _ _ _ V_x Eq_z) as [y [V_y [ P_xy <- ]]].
+        constructor.
+        + MatchState.solve.
+        + dependent destruction P_xy. assumption.
     Qed.
   End Monotony.
 
   Module Safety.
-    Definition SafeContinuation (x0: MatchState) (dir: direction) (c: MatcherContinuation) :=
+(*     Definition SafeContinuation (x0: MatchState) (str: list Character) (c: MatcherContinuation) (dir: direction) :=
       forall x,
-          Valid x
-      ->  progress dir x0 (fsuccess x) 
-      ->  c x <> assertion_failed.
-    Definition SafeMatcher (dir: direction) (m: Matcher) :=
-      forall x c,
-          Valid x
-      ->  SafeContinuation x dir c
-      ->  m x c <> assertion_failed.
+        (* For any valid state *)
+        MatchState.Valid str x ->
+        (* which is a progress from the threshold state *)
+        progress dir x0 (Success (Some x)) ->
+        (* Then the overall computation does not trigger an assertion *)
+        c x <> assertion_failed. *)
+    Definition SafeMatcher (str: list Character) (rer: RegExp) (m: Matcher) (dir: direction) := forall x c,
+      (* For any valid state *)
+      MatchState.Valid str rer x ->
+      (* If the overall computation runs out of fuel *)
+      m x c = assertion_failed ->
+      (* There is an intermediate value y that was produced by m and then passed to c which then ran out of fuel. *)
+      exists y, MatchState.Valid str rer y /\ progress dir x (Success (Some y)) /\ c y = assertion_failed.
     #[export]
-    Hint Unfold SafeContinuation SafeMatcher: Warblre.
+    Hint Unfold (*SafeContinuation*) SafeMatcher: Warblre.
 
-    Lemma continuation_weakening: forall x x' dir (c: MatcherContinuation), progress dir x (fsuccess x')
-      -> SafeContinuation x dir c -> SafeContinuation x' dir c.
-    Proof. intros. intros y Vy Pxy. apply H0; try assumption. Progress.saturate. Qed.
+(*     Lemma continuation_weakening: forall x x' str dir (c: MatcherContinuation), progress dir x (Success (Some x'))
+      -> SafeContinuation x str c dir -> SafeContinuation x' str c dir.
+    Proof. intros. intros y V_y P_x'_y. apply H0; try assumption. Progress.saturate. Qed. *)
 
-    Lemma repeatMatcher: forall fuel dir m min max greedy captures,
-      SafeMatcher dir m -> SafeMatcher dir (fun x c => repeatMatcher' m min max greedy x c captures fuel).
+    Ltac search := lazymatch goal with
+    | [ H: Failure _ = assertion_failed |- _ ] => try rewrite -> H in *; clear H; search
+    | [ H: ?c ?y = assertion_failed |- exists x, MatchState.Valid _ _ x /\ progress ?dir _ _ /\ ?c x = assertion_failed ] =>
+      exists y; split_conjs;
+      [ try Progress.solve
+      | try solve [Progress.saturate]
+      | apply H ]
+    end.
+
+    Lemma repeatMatcher: forall dir m min max greedy captures rer str,
+      Captures.Valid rer captures ->
+      SafeMatcher str rer m dir ->
+      SafeMatcher str rer (fun x c => repeatMatcher m min max greedy x c captures) dir.
     Proof.
-      induction fuel; intros; intros x c Vx Sc; cbn; try easy.
-      focus § _ (_ [] _) § auto destruct.
-      - apply Sc; try assumption. apply Progress.refl.
-      - apply H; try Progress.solve.
-        intros y Vy Pxy. focus § _ (_ [] _) § auto destruct.
-        apply IHfuel with (dir := dir); try assumption.
-        apply Safety.continuation_weakening with (x := x); try assumption.
-        Progress.solve.
-      - apply H; try Progress.solve.
-        intros y Vy Pxy. focus § _ (_ [] _) § auto destruct.
-        apply IHfuel with (dir := dir); try assumption.
-        apply Safety.continuation_weakening with (x := x); try assumption.
-        Progress.solve.
-      - rewrite <- AutoDest_2. apply Sc; try assumption. apply Progress.refl.
-      - apply Sc; try assumption. apply Progress.refl.
-      - rewrite <- AutoDest_2.
-        apply H; try Progress.solve.
-        intros y Vy Pxy. focus § _ (_ [] _) § auto destruct.
-        apply IHfuel with (dir := dir); try assumption.
-        apply Safety.continuation_weakening with (x := x); try assumption.
-        Progress.solve.
+      assert (Ind: forall fuel dir m min max greedy captures rer str,
+        Captures.Valid rer captures ->
+        SafeMatcher str rer m dir ->
+        SafeMatcher str rer (fun x c => repeatMatcher' m min max greedy x c captures fuel) dir). {
+          induction fuel; intros dir m min max greedy captures rer str V_captures S_m x c V_x Eq_af; cbn in Eq_af; try easy.
+          focus § _ [] _ § auto destruct in Eq_af.
+          - search.
+          - apply S_m in Eq_af as [ y0 [ V_y0 [ P_x_y0 Eq_af ]]]; try MatchState.solve.
+            + focus § _ [] _ § auto destruct in Eq_af.
+              apply (IHfuel _ _ _ _ greedy captures _ str V_captures S_m _ c V_y0) in Eq_af as [ y1 [ V_y1 [ P_y0_y1 Eq_af ]]].
+              search.
+          - apply S_m in Eq_af as [ y0 [ V_y0 [ P_x_y0 Eq_af ]]]; try MatchState.solve.
+            focus § _ [] _ § auto destruct in Eq_af.
+            apply (IHfuel _ _ _ _ greedy captures _ str V_captures S_m _ c V_y0) in Eq_af as [ y1 [ V_y1 [ P_y0_y1 Eq_af ]]].
+            search.
+          - rewrite <- Eq_af. search.
+          - search.
+          - injection Eq_af as ->.
+            apply S_m in AutoDest_3 as [ y0 [ V_y0 [ P_x_y0 Eq_af ]]]; try MatchState.solve.
+            focus § _ [] _ § auto destruct in Eq_af.
+            apply (IHfuel _ _ _ _ greedy captures _ str V_captures S_m _ c V_y0) in Eq_af as [ y1 [ V_y1 [ P_y0_y1 Eq_af ]]].
+            search.
+          - injection Eq_af as ->.
+            apply List.Update.Nat.Batch.failure_bounds in AutoDest_0. unfold Captures.Valid in V_captures.
+            destruct V_x as [ _ [ _ [ VCL_x _ ]]]. rewrite -> VCL_x in *. contradiction.
+      }
+      intros dir m min max greedy captures rer str H H0 x c H1 H2. specialize Ind with (1 := H) (2 := H0).
+      unfold repeatMatcher. unfold SafeMatcher in Ind.
+      apply Ind with (1 := H1) (2 := H2).
+      Qed.
+
+    Lemma characterSetMatcher: forall str rer A invert dir,
+      SafeMatcher str rer (characterSetMatcher rer A invert dir) dir.
+    Proof.
+      intros str rer A invert dir x c Vx Eq_oof.
+      unfold characterSetMatcher in Eq_oof. focus § _ [] _ § auto destruct in Eq_oof.
+      - search.
+        + Zhelper. MatchState.solve_with lia.
+        + apply Progress.step. lia.
+      - injection Eq_oof as ->. apply List.Exists.failure_kind in AutoDest_1.
+        destruct AutoDest_1 as [ i [ v [ Indexed_A_i Eq_v_s ]]].
+        discriminate.
+      - injection Eq_oof as ->. boolean_simplifier. Zhelper.
+        destruct Vx as [ Eq_str [ [ ? ? ] _ ]].
+        destruct dir.
+        + assert (Z.min (MatchState.endIndex x) (MatchState.endIndex x + 1) = MatchState.endIndex x)%Z as Tmp by lia.
+          rewrite -> Tmp in *; clear Tmp.
+          apply List.Indexing.Int.failure_bounds in AutoDest_0 as [ ? | ? ]; lia.
+        + assert (Z.min (MatchState.endIndex x) (MatchState.endIndex x - 1) = MatchState.endIndex x - 1)%Z as Tmp by lia.
+          rewrite -> Tmp in *; clear Tmp.
+          rewrite -> Eq_str in *.
+          apply List.Indexing.Int.failure_bounds in AutoDest_0 as [ ? | ? ]; try lia.
     Qed.
 
-    Lemma compileSubPattern: forall r dir rer, SafeMatcher dir (compileSubPattern r rer dir).
+    Lemma positiveLookaroundMatcher: forall m str rer dir dir',
+      IntermediateValue.HonoresContinuation str rer m dir' ->
+      SafeMatcher str rer m dir' ->
+      SafeMatcher str rer (Definitions.PositiveLookaround.matcher m) dir.
     Proof.
-      induction r; cbn; intros dir rer x c Vx Sc;
-      focus § _ (_ [] _) § auto destruct.
-      - apply Sc; try Progress.solve.
-      - apply Sc; try Progress.solve.
-      - apply Indexing.failure_kind in AutoDest_0.
-        rewrite -> Indexing.failure_bounds in *.
-        unfold Valid in *. destruct dir; cbn in *; Zhelper; try lia.
-      - apply IHr2; assumption.
-      - rewrite <- AutoDest_. apply IHr1; assumption.
-      - apply Safety.repeatMatcher with (x := x) (dir := dir); try assumption.
-        intros. apply IHr; try assumption.
-      - intros.
-        apply IHr1; try assumption.
-        intros y Vy Pxy. apply IHr2; try assumption.
-        apply Safety.continuation_weakening with (x := x); assumption.
-      - intros.
-        apply IHr2 with (x := x); try assumption.
-        intros y Vy Pxy. apply IHr1; try assumption.
-        apply Safety.continuation_weakening with (x := x); assumption.
-      - apply IHr with (x := x); try assumption.
-        intros y Vy Pxy. focus § _ (_ [] _) § auto destruct.
-        + apply Sc; Progress.solve.
-        + focus § _ [] _ § auto destruct in AutoDest_;
-            destruct dir; try discriminate; inversion Pxy; inversion H3; Zhelper; lia.
-      - apply Sc; Progress.solve.
-      - rewrite <- AutoDest_. apply IHr; try assumption.
-        easy.
-      - apply Sc; Progress.solve.
-      - rewrite <- AutoDest_. apply IHr; try assumption.
-        easy.
-      - apply Sc; Progress.solve.
-      - rewrite <- AutoDest_. apply IHr; try assumption.
-        easy.
-      - apply Sc; Progress.solve.
-      - rewrite <- AutoDest_. apply IHr; try assumption.
-        easy.
+      intros m str rer dir dir' HC_m S_m. intros x c V_x Eq_af.
+      unfold Definitions.PositiveLookaround.matcher in *.
+      focus § _ [] _ § auto destruct in Eq_af.
+      + specialize (HC_m _ _ _ V_x AutoDest_) as [ y0 [ V_y0 [ P_x_y0 Eq_y0 ]]].
+        search.
+      + injection Eq_af as ->.
+        specialize (S_m _ _ V_x AutoDest_) as [ y0 [ V_y0 [ P_x_y0 Eq_y0 ]]].
+        discriminate.
     Qed.
 
-    Theorem compilePattern: forall r rer input i, 0 <= i <= (length input) -> compilePattern r rer input i <> assertion_failed.
+    Lemma negativeLookaroundMatcher: forall m str rer dir dir',
+      SafeMatcher str rer m dir' ->
+      SafeMatcher str rer (Definitions.NegativeLookaround.matcher m) dir.
     Proof.
-      intros. delta compilePattern. cbn.
+      intros m str rer dir dir' S_m. intros x c V_x Eq_af.
+      unfold Definitions.NegativeLookaround.matcher in *.
+      focus § _ [] _ § auto destruct in Eq_af.
+      + search.
+      + injection Eq_af as ->.
+        specialize (S_m _ _ V_x AutoDest_) as [ y0 [ V_y0 [ P_x_y0 Eq_y0 ]]].
+        discriminate.
+    Qed.
+
+    Lemma backreferenceMatcher: forall str rer n dir,
+      n < RegExp.capturingGroupsCount rer ->
+      SafeMatcher str rer (backreferenceMatcher rer n dir) dir.
+    Proof.
+      intros str rer n dir Bound_n x c Vx Eq_af.
+      unfold backreferenceMatcher in Eq_af. focus § _ [] _ § auto destruct in Eq_af.
+      - search.
+      - search.
+        + destruct dir; cbn in *; MatchState.solve_with ltac:(cbn in *; lia).
+        + apply Progress.step. MatchState.normalize. cbn in *. lia.
+      - injection Eq_af as ->. Zhelper.
+        apply List.Exists.failure_kind in AutoDest_3.
+        destruct AutoDest_3 as [ i [ j [ Eq_indexed Eq_af ]]].
+        pose proof Eq_indexed as Tmp. apply List.Range.indexing in Tmp as ->.
+        apply List.Indexing.Int.success_bounds in Eq_indexed as Bounds_i. clear Eq_indexed.
+        destruct Vx as [ Eq_str [ [ ? ? ] [ _ V_t ]]]. specialize (V_t _ _ AutoDest_). dependent destruction V_t.
+        rename s into t_s, e into t_e, H into Ineq_t, H0 into IO_t_s, H1 into IO_t_e.
+        MatchState.normalize. cbn in *. rewrite -> List.Range.length in *.
+        focus § _ [] _ § auto destruct in Eq_af; injection Eq_af as ->.
+        + destruct dir.
+          * apply List.Indexing.Int.failure_bounds in AutoDest_1 as [ ? | ? ]; lia.
+          * apply List.Indexing.Int.failure_bounds in AutoDest_1 as [ ? | ? ]; lia.
+        + destruct dir.
+          * apply List.Indexing.Int.failure_bounds in AutoDest_0 as [ ? | ? ]; lia.
+          * apply List.Indexing.Int.failure_bounds in AutoDest_0 as [ ? | ? ]; lia.
+      - injection Eq_af as ->.
+        apply List.Indexing.Nat.failure_bounds in AutoDest_.
+        destruct Vx as [ _ [ _ [ Tmp _ ]]]; rewrite -> Tmp in *; clear Tmp.
+        lia.
+    Qed.
+
+    Lemma compileSubPattern: forall r dir str rer,
+      Groups.Bounded r (RegExp.capturingGroupsCount rer) ->
+      SafeMatcher str rer (compileSubPattern r rer dir) dir.
+    Proof.
+      induction r; cbn; intros dir str rer GB_r; dependent destruction GB_r.
+      - intros x c Vx Sc. search.
+      - apply characterSetMatcher.
+      - intros x c Vx Sc.
+        focus § _ [] _ § auto destruct in Sc.
+        + unfold SafeMatcher in IHr2.
+          specialize IHr2 with (1 := GB_r2) (dir := dir) (str := str) (x := x) (c := c). fforward.
+          destruct IHr2 as [ ? [ ? [ ? ? ]]]. search.
+        + injection Sc as ->.
+          unfold SafeMatcher in IHr1.
+          specialize IHr1 with (1 := GB_r1) (dir := dir) (str := str) (x := x) (c := c). fforward.
+          destruct IHr1 as [ ? [ ? [ ? ? ]]]. search.
+      - apply repeatMatcher.
+        + apply Groups.capturesWithinValid. assumption.
+        + apply IHr. assumption.
+      - intros x c V_x S_c. destruct dir.
+        + specialize (IHr1 _ _ _ GB_r1 _ _ V_x S_c) as [ y0 [ V_y0 [ P_x_y0 Eq_y0 ]]].
+          specialize (IHr2 _ _ _ GB_r2 _ _ V_y0 Eq_y0) as [ y1 [ V_y1 [ P_x_y1 Eq_y1 ]]].
+          search.
+        + specialize (IHr2 _ _ _ GB_r2 _ _ V_x S_c) as [ y0 [ V_y0 [ P_x_y0 Eq_y0 ]]].
+          specialize (IHr1 _ _ _ GB_r1 _ _ V_y0 Eq_y0) as [ y1 [ V_y1 [ P_x_y1 Eq_y1 ]]].
+          search.
+      - intros x c V_x Eq_af.
+        specialize (IHr _ _ _ GB_r _ _ V_x Eq_af) as [ y0 [ V_y0 [ P_x_y0 Eq_y0 ]]].
+        focus § _ [] _ § auto destruct in Eq_y0.
+        + focus § _ [] _ § auto destruct in AutoDest_.
+          * search. MatchState.solve_with lia.
+          * search. MatchState.solve_with lia.
+        + injection Eq_y0 as ->. apply List.Update.Nat.One.failure_bounds in AutoDest_0.
+          MatchState.solve_with lia.
+        + injection Eq_y0 as ->.
+          focus § _ [] _ § auto destruct in AutoDest_; destruct dir; try discriminate.
+          * Zhelper. MatchState.normalize.
+            dependent destruction P_x_y0.
+            dependent destruction H1. cbn in *.
+            lia.
+          * Zhelper.
+            dependent destruction P_x_y0.
+            dependent destruction H1. cbn in *.
+            lia.
+      - apply positiveLookaroundMatcher with (dir' := forward).
+        + apply IntermediateValue.compileSubPattern.
+        + apply IHr. assumption.
+      - apply negativeLookaroundMatcher with (dir' := forward). apply IHr. assumption.
+      - apply positiveLookaroundMatcher with (dir' := backward).
+        + apply IntermediateValue.compileSubPattern.
+        + apply IHr. assumption.
+      - apply negativeLookaroundMatcher with (dir' := backward). apply IHr. assumption.
+      - apply backreferenceMatcher. assumption.
+    Qed.
+
+    Theorem compilePattern: forall r rer input i,
+      Groups.Bounded r (RegExp.capturingGroupsCount rer) ->
+      0 <= i <= (length input) ->
+      compilePattern r rer input i <> assertion_failed.
+    Proof.
+      intros r rer input i GB Bounds_i. delta compilePattern. cbn.
       focus § _ (_ [] _) § auto destruct.
       - hypotheses_reflector. spec_reflector Nat.leb_spec0. contradiction.
-      - apply Safety.compileSubPattern.
-        + hypotheses_reflector. constructor; cbn; lia.
-        + easy.
+      - remember (match_state input i (List.repeat None (RegExp.capturingGroupsCount rer))) as x eqn:Eq_x.
+        pose proof (Safety.compileSubPattern _ forward input _ GB x (fun y => y)) as Falsum.
+        assert (MatchState.Valid input rer x) as V_x. {
+          subst x. apply MatchState.valid_init. lia.
+        }
+        focus § _ (_ [] _) § do (fun t => destruct t as [ | f ]; try easy; destruct f; try easy).
+        fforward. destruct Falsum as [ ? [ _ [ _ ? ]]].
+        subst. discriminate.
     Qed.
   End Safety.
 
   Module Termination.
-    Definition TerminatingMatcher (m: Matcher) (dir: direction) :=
-      forall x c, Valid x -> m x c = out_of_fuel -> exists y, Valid y /\ progress dir x (fsuccess y) /\ c y = out_of_fuel.
+    Definition TerminatingMatcher (str: list Character) (rer: RegExp) (m: Matcher) (dir: direction) := forall x c,
+      (* For any valid state *)
+      MatchState.Valid str rer x ->
+      (* If the overall computation runs out of fuel *)
+      m x c = out_of_fuel ->
+      (* There is an intermediate value y that was produced by m and then passed to c which then ran out of fuel. *)
+      exists y, MatchState.Valid str rer y /\ progress dir x (Success (Some y)) /\ c y = out_of_fuel.
     #[export]
     Hint Unfold TerminatingMatcher: Warblre.
 
@@ -385,45 +777,95 @@ Module Correctness.
     #[export]
     Hint Unfold fuelBound remainingChars : Warblre.
 
-    Lemma repeatMatcherFuel_satisfies_bound: forall min x dir, Valid x -> fuelBound min x dir <= repeatMatcherFuel min x.
-    Proof. intros. autounfold with Warblre in *. unfold Valid in *. destruct dir; cbn; lia. Qed.
+    Lemma repeatMatcherFuel_satisfies_bound: forall min x str rer dir, MatchState.Valid str rer x -> fuelBound min x dir <= repeatMatcherFuel min x.
+    Proof. intros. autounfold with Warblre in *. destruct H as [ <- [ [ Bounds_Ei_x_low Bounds_Ei_x_high ] VC_x ] ]. destruct dir; cbn; lia. Qed.
 
-    Lemma fuelDecreases_min: forall dir min min' x x' b, 
-      min' < min -> progress dir x (fsuccess x') 
-      -> fuelBound min x dir <= S b -> fuelBound min' x' dir <= b.
+    Lemma fuelDecreases_min: forall dir min min' x x' b,
+      min' < min -> progress dir x (Success (Some x')) -> fuelBound min x dir <= S b -> fuelBound min' x' dir <= b.
     Proof.
       intros. autounfold with Warblre in *. inversion H0; destruct dir; inversion H6; subst.
       - rewrite -> H3 in *. lia.
       - lia.
     Qed.
 
-    Lemma fuelDecreases_progress: forall dir min x x' b, 
-      progress dir x (fsuccess x') -> ((MatchState.endIndex x) =? (MatchState.endIndex x'))%Z = false
-      -> Valid x -> Valid x'
-      -> fuelBound min x dir <= S b -> fuelBound min x' dir <= b.
+    Lemma fuelDecreases_progress: forall dir str rer min x x' b,
+      progress dir x (Success (Some x')) ->
+      ((MatchState.endIndex x) =? (MatchState.endIndex x'))%Z = false ->
+      MatchState.Valid str rer x ->
+      MatchState.Valid str rer x' ->
+      fuelBound min x dir <= S b ->
+      fuelBound min x' dir <= b.
     Proof.
-      intros. autounfold with Warblre in *. destruct H1. destruct H2. spec_reflector Z.eqb_spec.
-      destruct dir; inversion H.
-      - inversion H10. subst. rewrite -> H7 in *. lia.
-      - inversion H10. lia.
+      intros dir str rer min x x' b P_x_x' Neq_Eis [ <- [ [ Bei_x_l Bei_x_h ] VC_x ] ] [ <- [ [ B_Ei_x'_l B_Ei_x'_h ] VC_x' ] ] Ineq_fuel.
+      dependent destruction P_x_x'. rename H into Eq_inp_x_x', H0 into Dp_x_x'.
+      unfold fuelBound, remainingChars in *.
+      rewrite <- Eq_inp_x_x' in *.
+      spec_reflector Z.eqb_spec.
+      dependent destruction Dp_x_x'; lia.
     Qed.
 
     Ltac search := lazymatch goal with
     | [ H: Failure _ = out_of_fuel |- _ ] => try rewrite -> H in *; clear H; search
-    | [ H: ?c ?y = out_of_fuel |- exists x, Valid x /\ progress ?dir _ _ /\ ?c x = out_of_fuel ] =>
+    | [ H: ?c ?y = out_of_fuel |- exists x, MatchState.Valid _ _ x /\ progress ?dir _ _ /\ ?c x = out_of_fuel ] =>
       exists y; split; [ | split ];
-      [ try solve [Progress.saturate]
+      [ try Progress.solve
       | try solve [Progress.saturate]
       | apply H ]
     end.
 
-    Lemma repeatMatcher': forall fuel m min max greedy captures x c dir, fuelBound min x dir <= fuel -> Valid x ->
-      TerminatingMatcher m dir ->
+    Lemma repeatMatcher': forall fuel m min max greedy captures x c dir str rer,
+      fuelBound min x dir <= fuel ->
+      MatchState.Valid str rer x ->
+      TerminatingMatcher str rer m dir ->
       repeatMatcher' m min max greedy x c captures fuel = out_of_fuel ->
-      exists y, Valid y /\ progress dir x (fsuccess y) /\ c y = out_of_fuel.
+      exists y,
+        MatchState.Valid str rer y /\ progress dir x (Success (Some y)) /\ c y = out_of_fuel.
     Proof.
-      induction fuel; intros m min max greedy captures x c dir INEQ_fuel Vx Tm Falsum.
-      - autounfold with Warblre in *. lia.
+      (* The 'recursive' case (i.e. when min is not zero or the endIndex is different from last iteration) *)
+  (*     assert (forall x s c str fuel dir m min max greedy groups,
+        MatchState.Valid str x ->
+        List.Updating.batch_updating (MatchState.captures x) groups None = Success s ->
+        TerminatingMatcher str m dir ->
+        (forall dir m min max greedy groups,
+          TerminatingMatcher str m dir ->
+          TerminatingMatcher str (Definitions.RepeatMatcher.matcher m min max greedy groups fuel) dir) ->
+        (m (match_state (MatchState.input x) (MatchState.endIndex x) s)
+          (Definitions.RepeatMatcher.continuation x c m min max greedy groups fuel) = out_of_fuel) ->
+        exists y : MatchState,
+          MatchState.Valid str y /\ progress dir x (Success (Some y)) /\ c y = out_of_fuel
+      ) as Rec. {
+        intros x s c str fuel dir m min max greedy groups V_x Eq_s Tm IH Eq_rec.
+        apply Tm in Eq_rec; try Progress.solve. destruct Eq_rec as [ y [ Vy [ P_x_y Eq_rec ] ] ].
+        (focus § _ [] _ § auto destruct in Eq_rec). boolean_simplifier.
+        destruct (PeanoNat.Nat.eq_dec min 0).
+        - assert(FD: fuelBound 0 y dir <= fuel). {
+            (focus § _ [] _ § do (fun t => apply fuelDecreases_progress with (str := str) (x := t)) in P_x_y); try Progress.solve.
+            MatchState.normalize. spec_reflector Z.eqb_spec. congruence.
+          }
+          admit.
+        - assert(FD: fuelBound (min - 1) y dir <= fuel). {
+            apply fuelDecreases_min with (min := min) (x := x); try Progress.solve.
+            + lia.
+            + admit.
+          }
+          admit.
+          (* specialize IH with (1 := FD) (2 := Vy) (3 := Tm) (4 := Eq_rec). clear Eq_rec.
+          destruct IH as [ z [ Vz [ Pyz Falsum ] ] ].
+          search. *)
+        
+        (*unfold TerminatingMatcher in Tm, IH.
+        specialize IH with (1 := Tm).
+        focus § _ (_ _ []) _ § remember as d in Eq_rec.
+        specialize HCm with (2 := Eq_rec).
+        fforward HCm as [ y0 [ Vy0 [ Pxy0 Eq_dy0 ]] ] by MatchState.solve.
+        rewrite -> Heqd in Eq_dy0. unfold Definitions.RepeatMatcher.continuation in Eq_dy0.
+        focus § _ [] _ § auto destruct in Eq_dy0.
+        specialize IH with (2 := Eq_dy0). fforward IH as [ y1 [ Vy1 [ Py0y1 Eq_cy1 ]]].
+        search.*)
+      } *)
+    
+      induction fuel; intros m min max greedy captures x c dir str rer Ineq_fuel Vx Tm Falsum.
+      - clear -Ineq_fuel. unfold fuelBound, remainingChars in *. lia.
       - cbn in Falsum.
         (focus § _ [] _ § auto destruct in Falsum).
         + search.
@@ -440,7 +882,7 @@ Module Correctness.
           (focus § _ [] _ § auto destruct in Falsum).
           boolean_simplifier. spec_reflector Nat.eqb_spec. subst.
           assert(FD: fuelBound 0 y dir <= fuel). {
-            (focus § _ [] _ § do (fun t => apply fuelDecreases_progress with (x := t)) in Pxy); try Progress.solve.
+            (focus § _ [] _ § do (fun t => apply fuelDecreases_progress with (str := str) (rer := rer) (x := t)) in Pxy); try Progress.solve.
             MatchState.normalize. spec_reflector Z.eqb_spec. congruence.
           }
           specialize IHfuel with (1 := FD) (2 := Vy) (3 := Tm) (4 := Falsum). clear Falsum.
@@ -448,57 +890,136 @@ Module Correctness.
           search.
         + search.
         + search.
-        + rewrite -> Falsum in *. clear Falsum. apply Tm in AutoDest_2; try Progress.solve. destruct AutoDest_2 as [ y [ Vy [ Pxy Falsum ] ] ].
+        + rewrite -> Falsum in *. clear Falsum. apply Tm in AutoDest_3; try Progress.solve. destruct AutoDest_3 as [ y [ Vy [ Pxy Falsum ] ] ].
           (focus § _ [] _ § auto destruct in Falsum).
           boolean_simplifier. spec_reflector Nat.eqb_spec. subst.
           assert(FD: fuelBound 0 y dir <= fuel). {
-            (focus § _ [] _ § do (fun t => apply fuelDecreases_progress with (x := t)) in Pxy); try Progress.solve.
+            (focus § _ [] _ § do (fun t => apply fuelDecreases_progress with (str := str) (rer := rer) (x := t)) in Pxy); try Progress.solve.
             MatchState.normalize. spec_reflector Z.eqb_spec. congruence.
           }
           specialize IHfuel with (1 := FD) (2 := Vy) (3 := Tm) (4 := Falsum). clear Falsum.
           destruct IHfuel as [ z [ Vz [ Pyz Falsum ] ] ].
           search.
+        + injection Falsum as ->.
+          apply List.Update.Nat.Batch.failure_is_assertion in AutoDest_0.
+          discriminate.
     Qed.
 
-    Lemma repeatMatcher: forall m min max greedy captures dir,
-      TerminatingMatcher m dir -> TerminatingMatcher (fun x c => repeatMatcher m min max greedy x c captures) dir.
-    Proof. unfold Semantics.repeatMatcher, TerminatingMatcher. intros.
-      pose proof repeatMatcher' as Tmp. specialize Tmp with (4 := H1). apply Tmp; try easy.
-      apply repeatMatcherFuel_satisfies_bound. assumption.
-    Qed.
-
-    Lemma compileSubPattern: forall r rer dir, TerminatingMatcher (compileSubPattern r rer dir) dir.
+    Lemma repeatMatcher: forall m min max greedy captures str rer dir,
+      TerminatingMatcher str rer m dir ->
+      TerminatingMatcher str rer (fun x c => repeatMatcher m min max greedy x c captures) dir.
     Proof.
-      induction r; intros rer dir; cbn -[Semantics.repeatMatcher];
+      unfold Semantics.repeatMatcher, TerminatingMatcher. intros m min max greedy captures str rer dir Tm x c V_x Eq_oof.
+      apply repeatMatcher' with (4 := Eq_oof); try easy.
+      apply repeatMatcherFuel_satisfies_bound with (str := str) (rer := rer).
+      assumption.
+    Qed.
+
+    Lemma characterSetMatcher: forall str rer A invert dir,
+      TerminatingMatcher str rer (characterSetMatcher rer A invert dir) dir.
+    Proof.
+      intros str rer A invert dir x c Vx Eq_oof.
+      unfold characterSetMatcher in Eq_oof. focus § _ [] _ § auto destruct in Eq_oof.
+      - search.
+        + Zhelper. MatchState.solve_with lia.
+        + apply Progress.step. lia.
+      - injection Eq_oof as ->. apply List.Exists.failure_kind in AutoDest_1.
+        destruct AutoDest_1 as [ i [ v [ Indexed_A_i Eq_v_s ]]].
+        discriminate.
+      - injection Eq_oof as ->.
+        pose proof (@List.Indexing.Int.failure_kind Character) as Falsum. specialize Falsum  with (1 := AutoDest_0).
+        cbn in *. congruence.
+    Qed.
+
+    Lemma positiveLookaroundMatcher: forall m str rer dir dir',
+      IntermediateValue.HonoresContinuation str rer m dir' ->
+      TerminatingMatcher str rer m dir' ->
+      TerminatingMatcher str rer (Definitions.PositiveLookaround.matcher m) dir.
+    Proof.
+      intros m str rer dir dir' HC_m S_m. intros x c V_x Eq_oof.
+      unfold Definitions.PositiveLookaround.matcher in *.
+      focus § _ [] _ § auto destruct in Eq_oof.
+      + specialize (HC_m _ _ _ V_x AutoDest_) as [ y0 [ V_y0 [ P_x_y0 Eq_y0 ]]].
+        search.
+      + injection Eq_oof as ->.
+        specialize (S_m _ _ V_x AutoDest_) as [ y0 [ V_y0 [ P_x_y0 Eq_y0 ]]].
+        discriminate.
+    Qed.
+
+    Lemma negativeLookaroundMatcher: forall m str rer dir dir',
+      TerminatingMatcher str rer m dir' ->
+      TerminatingMatcher str rer (Definitions.NegativeLookaround.matcher m) dir.
+    Proof.
+      intros m str rer dir dir' S_m. intros x c V_x Eq_oof.
+      unfold Definitions.NegativeLookaround.matcher in *.
+      focus § _ [] _ § auto destruct in Eq_oof.
+      + search.
+      + injection Eq_oof as ->.
+        specialize (S_m _ _ V_x AutoDest_) as [ y0 [ V_y0 [ P_x_y0 Eq_y0 ]]].
+        discriminate.
+    Qed.
+
+    Lemma backreferenceMatcher: forall str rer n dir,
+      TerminatingMatcher str rer (backreferenceMatcher rer n dir) dir.
+    Proof.
+      unfold TerminatingMatcher. intros str rer n dir x c Vx Eq_oof.
+      unfold backreferenceMatcher in Eq_oof. focus § _ [] _ § auto destruct in Eq_oof.
+      - search.
+      - search.
+        + destruct dir; cbn in *; MatchState.solve_with ltac:(cbn in *; lia).
+        + apply Progress.step. MatchState.normalize. cbn in *. lia.
+      - injection Eq_oof as ->.
+        apply List.Exists.failure_kind in AutoDest_3.
+        destruct AutoDest_3 as [ i [ j [ Eq_indexed Eq_oof ]]].
+        focus § _ [] _ § auto destruct in Eq_oof.
+        + injection Eq_oof as ->.
+          pose proof (@List.Indexing.Int.failure_kind Character) as Falsum. specialize Falsum  with (1 := AutoDest_4).
+          cbn in *. congruence.
+        + injection Eq_oof as ->.
+          pose proof (@List.Indexing.Int.failure_kind Character) as Falsum. specialize Falsum  with (1 := AutoDest_3).
+          cbn in *. congruence.
+      - injection Eq_oof as ->.
+        pose proof @List.Indexing.Nat.failure_kind as Falsum. specialize Falsum  with (1 := AutoDest_).
+        cbn in *. congruence.
+    Qed.
+
+    Lemma compileSubPattern: forall r rer dir str, TerminatingMatcher str rer (compileSubPattern r rer dir) dir.
+    Proof.
+      induction r; intros rer dir str; cbn -[Semantics.repeatMatcher];
       focus § _ [] _ § auto destruct.
       - intros x c Vx H. search.
-      - intros x c Vx H. autounfold with Warblre in *. focus § _ [] _ § auto destruct in H.
-        + search.
-        + apply Indexing.failure_is_assertion in AutoDest_0. simpl in AutoDest_0. congruence.
+      - apply characterSetMatcher.
       - intros x c Vx H. autounfold with Warblre in *. focus § _ [] _ § auto destruct in H; repeat (specialize_once; bookkeeper); search.
       - apply repeatMatcher. apply IHr.
-      - intros x c Vx H. autounfold with Warblre in *. repeat (auto_specialize; Coq.Program.Tactics.destruct_conjs). search.
-      - intros x c Vx H. autounfold with Warblre in *. repeat (auto_specialize; Coq.Program.Tactics.destruct_conjs). search.
-      - intros x c Vx H. autounfold with Warblre in *. repeat (auto_specialize; Coq.Program.Tactics.destruct_conjs).
-        focus § _ [] _ § auto destruct in H4.
-        + search.
-        + focus § _ [] _ § auto destruct in AutoDest_; congruence.
       - intros x c Vx H. autounfold with Warblre in *.
-        focus § _ [] _ § auto destruct in H.
-        + search.
-        + rewrite -> H in *; clear H. repeat (auto_specialize; Coq.Program.Tactics.destruct_conjs). discriminate.
+        specialize IHr1 with (1 := Vx) (2 := H) as [ y0 [ Vy0 [ P_x_y0 Eq_oof0 ]]].
+        specialize IHr2 with (1 := Vy0) (2 := Eq_oof0) as [ y1 [ Vy1 [ P_y0_y1 Eq_oof1 ]]].
+        search.
       - intros x c Vx H. autounfold with Warblre in *.
-        focus § _ [] _ § auto destruct in H.
-        + search.
-        + rewrite -> H in *; clear H. repeat (auto_specialize; Coq.Program.Tactics.destruct_conjs). discriminate.
-      - intros x c Vx H. autounfold with Warblre in *.
-        focus § _ [] _ § auto destruct in H.
-        + search.
-        + rewrite -> H in *; clear H. repeat (auto_specialize; Coq.Program.Tactics.destruct_conjs). discriminate.
-      - intros x c Vx H. autounfold with Warblre in *.
-        focus § _ [] _ § auto destruct in H.
-        + search.
-        + rewrite -> H in *; clear H. repeat (auto_specialize; Coq.Program.Tactics.destruct_conjs). discriminate.
+        specialize IHr2 with (1 := Vx) (2 := H) as [ y0 [ Vy0 [ P_x_y0 Eq_oof0 ]]].
+        specialize IHr1 with (1 := Vy0) (2 := Eq_oof0) as [ y1 [ Vy1 [ P_y0_y1 Eq_oof1 ]]].
+        search.
+      - intros x c Vx H. autounfold with Warblre in *. 
+        specialize IHr with (str := str) (1 := Vx) (2 := H).
+        destruct IHr as [ y [ Vy [ P_x_y Eq_oof ]]].
+        focus § _ [] _ § auto destruct in Eq_oof.
+        + search. MatchState.normalize; try MatchState.solve.
+          apply List.Update.Nat.One.prop_preservation with (ls := captures_y) (i := id) (v := s); try assumption.
+          focus § _ [] _ § auto destruct in AutoDest_; injection AutoDest_ as <-; constructor; solve [ assumption | lia ].
+        + rewrite -> List.Update.Nat.One.failure_kind with (f := f) in AutoDest_0 by assumption.
+          injection AutoDest_0 as <-. discriminate.
+        + focus § _ [] _ § auto destruct in AutoDest_.
+          * injection AutoDest_ as <-. discriminate.
+          * injection AutoDest_ as <-. discriminate.
+      - apply positiveLookaroundMatcher with (dir' := forward).
+        + apply IntermediateValue.compileSubPattern.
+        + apply IHr.
+      - apply negativeLookaroundMatcher with (dir' := forward). apply IHr.
+      - apply positiveLookaroundMatcher with (dir' := backward).
+        + apply IntermediateValue.compileSubPattern.
+        + apply IHr.
+      - apply negativeLookaroundMatcher with (dir' := backward). apply IHr.
+      - apply backreferenceMatcher.
     Qed.
 
     Lemma compilePattern: forall r rer input i, compilePattern r rer input i <> out_of_fuel.
@@ -507,17 +1028,17 @@ Module Correctness.
       focus § _ (_ [] _) § auto destruct.
       (focus § _ (_ [] _) § do (fun t => destruct t eqn:S)); try easy.
       destruct f; try easy.
-      pose proof compileSubPattern as Falsum. autounfold with Warblre in *. specialize Falsum with (2 := S).
-      focus § _ [] -> _ § do (fun t => assert(Valid t)) in Falsum.
-      - boolean_simplifier. spec_reflector Nat.leb_spec0. constructor; cbn; lia.
+      pose proof compileSubPattern as Falsum. autounfold with Warblre in *. specialize Falsum with (str := input) (2 := S).
+      focus § [] -> _ § do (fun t => assert(t)) in Falsum.
+      - apply MatchState.valid_init. boolean_simplifier. spec_reflector Nat.leb_spec0. lia.
       - specialize Falsum with (1 := H). Coq.Program.Tactics.destruct_conjs. discriminate.
     Qed.
 
-    From Coq Require Import Logic.FunctionalExtensionality.
+    (*From Coq Require Import Logic.FunctionalExtensionality.
     Definition TerminatingContinuation (c: MatcherContinuation) :=
       forall x, c x <> out_of_fuel.
-    Lemma repeatMatcher_fuelWeakening: forall fuelL fuelH (m: Matcher) min max greedy captures x c dir, fuelL <= fuelH ->
-      TerminatingMatcher m dir -> IntermediateValue.HonoresContinuation m dir -> TerminatingContinuation c ->
+    Lemma repeatMatcher_fuelWeakening: forall fuelL fuelH (m: Matcher) min max greedy captures x c dir str, fuelL <= fuelH ->
+      TerminatingMatcher str m dir -> IntermediateValue.HonoresContinuation str m dir -> TerminatingContinuation c ->
       Semantics.repeatMatcher' m min max greedy x c captures fuelL <> out_of_fuel -> 
       Semantics.repeatMatcher' m min max greedy x c captures fuelH = Semantics.repeatMatcher' m min max greedy x c captures fuelL.
     Proof.
@@ -551,6 +1072,6 @@ Module Correctness.
         + admit.
       - admit.
       - admit.
-    Abort.
+    Abort.*)
   End Termination.
 End Correctness.
