MECMAR/spec/Patterns.v
@@ -8,26 +8,65 @@ Module Patterns.
   | Question
   | RepExact (count: non_neg_integer)
   | RepPartialRange (min: non_neg_integer)
-  | RepRange (min: non_neg_integer) (max: non_neg_integer) (OK: (min <=? max)%nat = true).
+  | RepRange (min: non_neg_integer) (max: non_neg_integer) (inv: (min <=? max)%nat = true).
+
+(*   Module QuantifierPrefix.
+    Definition eqb (l r: QuantifierPrefix): {l = r} + {~ l = r}.
+    Proof. repeat decide equality. Defined.
+  End QuantifierPrefix. *)
 
   Inductive Quantifier :=
   | Greedy (p: QuantifierPrefix)
   | Lazy (p: QuantifierPrefix).
 
+(*   Module Quantifier.
+    Definition eqb (l r: Quantifier): {l = r} + {~ l = r}.
+    Proof. decide equality; apply QuantifierPrefix.eqb. Defined.
+  End Quantifier. *)
+
+(*   Module ClassAtom.
+    Definition eqb (l r: ClassAtom): {l = r} + {~ l = r}.
+    Proof. decide equality. apply Character.eqb. Defined.
+  End ClassAtom. *)
+
+  Inductive ClassRanges :=
+  | EmptyCR
+  | AtomChar (chr: Character)
+  (* Escapes: \b \w ...*)
+  (*| AtomHead (atom: ClassRanges) (rem: ClassRanges)
+  | RangeHead (from to: ClassRanges) (rem: ClassRanges)*).
+
+(*   Module ClassRanges.
+    Definition eqb (l r: ClassRanges): {l = r} + {~ l = r}.
+    Proof. decide equality; apply ClassAtom.eqb. Defined.
+  End ClassRanges. *)
+
+  Inductive CharacterClass :=
+  | PositiveCC (crs: ClassRanges)
+  | NegativeCC (crs: ClassRanges).
+
+(*   Module CharacterClass.
+    Definition eqb (l r: CharacterClass): {l = r} + {~ l = r}.
+    Proof. decide equality; apply ClassRanges.eqb. Defined.
+  End CharacterClass. *)
+
   Inductive Regex :=
   | Empty
-  | Char (A: CharSet) (invert: bool)
+  | Char (chr: Character)
   | Disjunction (r1 r2: Regex)
   | Quantified (r: Regex) (q: Quantifier)
   | Seq (r1 r2: Regex)
-  | Group (id: IdentifierName) (r: Regex)
+  | Group (id: nat) (r: Regex)
   (* Assertions: ^ $ \b \B *)
   | Lookahead (r: Regex)
   | NegativeLookahead (r: Regex)
   | Lookback (r: Regex)
   | NegativeLookbehind (r: Regex)
-  | BackReference (id: IdentifierName).
+  | BackReference (id: nat).
 
-  Implicit Types (r: Regex).
+(*   Module Regex.
+    Definition eqb (l r: Regex): {l = r} + {~ l = r}.
+    Proof. decide equality; (apply CharacterClass.eqb + apply Quantifier.eqb + (repeat decide equality)). Defined.
+  End Regex. *)
 End Patterns.
 Export Patterns.
