MECMAR/spec/StaticSemantics.v
@@ -1,27 +1,55 @@
+From Coq Require Import List.
 From Warblre Require Import Base Patterns.
 
 Module StaticSemantics.
+
+  Fixpoint pre_order_walk (r: Regex): list Regex := match r with
+  | Empty => r :: nil
+  | Char _ => r :: nil
+  | Disjunction r1 r2 => r :: (pre_order_walk r1 ++ pre_order_walk r2)
+  | Quantified r0 _ => r :: (pre_order_walk r0)
+  | Seq r1 r2 => r :: (pre_order_walk r1 ++ pre_order_walk r2)
+  | Group _ r0 => r :: (pre_order_walk r0)
+  | Lookahead r0 => r :: (pre_order_walk r0)
+  | NegativeLookahead r0 => r :: (pre_order_walk r0)
+  | Lookback r0 => r :: (pre_order_walk r0)
+  | NegativeLookbehind r0 => r :: (pre_order_walk r0)
+  | BackReference _ => r :: nil
+  end.
+
   (** 22.2.1.1 Static Semantics: Early Errors *)
   Inductive SyntaxStatus :=
   | SyntaxOK
   | SyntaxError.
 
   (** 22.2.1.2 Static Semantics: CountLeftCapturingParensWithin *)
-  Fixpoint capturingGroupsWithin (r: Regex): IdSet.t := match r with
-  | Empty => IdSet.empty
-  | Char _ _ => IdSet.empty
-  | Disjunction r1 r2 => IdSet.union (capturingGroupsWithin r1) (capturingGroupsWithin r2)
-  | Quantified r _ => capturingGroupsWithin r
-  | Seq r1 r2 => IdSet.union (capturingGroupsWithin r1) (capturingGroupsWithin r2)
-  | Group id r => IdSet.add id (capturingGroupsWithin r)
-  | Lookahead r => capturingGroupsWithin r
-  | NegativeLookahead r => capturingGroupsWithin r
-  | Lookback r => capturingGroupsWithin r
-  | NegativeLookbehind r => capturingGroupsWithin r
-  | BackReference _ => IdSet.empty
-  end.
+  Definition countLeftCapturingParensWithin (r: Regex): non_neg_integer := (*countLeftCapturingParensWithin_rec 0 r.*)
+    List.fold_left (fun acc r => match r with
+      | Group _ _ => acc + 1
+      | _ => acc
+      end) (pre_order_walk r) 0.
+
+  Definition capturingGroupsWithin (r: Regex): list nat :=
+    List.flat_map (fun r => match r with
+      | Group id _ => id :: nil
+      | _ => nil
+      end) (pre_order_walk r).
 
   (** 22.2.1.3 Static Semantics: CountLeftCapturingParensBefore *)
+(*   Fixpoint countLeftCapturingParensBefore_rec (target: Regex) (acc: non_neg_integer) (walk: list Regex): option non_neg_integer :=
+    match walk with
+    | nil => None
+    | iter :: walk' =>
+      if Regex.eqb target iter then
+        Some acc
+      else match iter with
+        | Group _ _ => countLeftCapturingParensBefore_rec target (S acc) walk'
+        | _ => countLeftCapturingParensBefore_rec target acc walk'
+        end
+    end.
+
+  Definition countLeftCapturingParensBefore (node pattern: Regex): option non_neg_integer :=
+    countLeftCapturingParensBefore_rec node 0 (pre_order_walk pattern). *)
 
   (** 22.2.1.4 Static Semantics: CapturingGroupNumber *)
 End StaticSemantics.
