MECMAR/utils/List.v
@@ -25,117 +25,420 @@ Module List.
 
   Definition empty {T: Type} := @nil T.
 
-  Module Indexing.
+  Module FoldResult.
+    Fixpoint fold_left_result0 {S T F: Type} (r: T -> S -> Result T F) (ls: list S) (racc: Result T F): Result T F := match ls with
+      | nil => racc
+      | s :: ls' => let! acc =<< racc in fold_left_result0 r ls' (r acc s)
+      end.
 
-    Definition indexing {T F: Type} (ls: list T) (i: Z) {failure: Result.AssertionError F}: Result.Result T F := match i with
-    | Z0 => Result.from_option_assertion (List.nth_error ls 0)
-    | Zpos i => Result.from_option_assertion (List.nth_error ls (Pos.to_nat i))
+    Definition fold_left_result {S T F: Type} (r: T -> S -> Result T F) (ls: list S) (zero: T): Result T F :=
+      fold_left_result0 r ls (Success zero).
+
+    Lemma zero_failure0 {S T F: Type}: forall (r: T -> S -> Result T F) (ls: list S) (f: F), fold_left_result0 r ls (Failure f) = (Failure f).
+    Proof. intros r ls f. destruct ls; reflexivity. Qed.
+
+    Lemma cons0 {S T F: Type}: forall (r: T -> S -> Result T F) (h: S) (t: list S) (zero: Result T F),
+      fold_left_result0 r (h :: t) zero = let! zero' =<< zero in fold_left_result0 r t (r zero' h).
+    Proof. intros r h t zero. reflexivity. Qed.
+
+    Lemma cons {S T F: Type}: forall (r: T -> S -> Result T F) (h: S) (t: list S) (acc: T),
+      fold_left_result r (h :: t) acc = let! acc' =<< r acc h in fold_left_result r t acc'.
+    Proof. intros r h t acc. destruct t. - cbn; destruct (r acc h); reflexivity. - cbn. reflexivity. Qed.
+  End FoldResult.
+
+  Local Notation "'Zextend' f" := (fun ls i => match i with
+    | Z0 => f ls 0%nat
+    | Zpos i => f ls (Pos.to_nat i)
     | Zneg _ => Result.assertion_failed
-    end.
+    end) (at level 0, only parsing).
 
-    Lemma of_nat {T F: Type} {failure: Result.AssertionError F}: forall (ls: list T) (i: nat), indexing ls (Z.of_nat i) = Result.from_option_assertion (List.nth_error ls i).
-    Proof. intros. destruct i. - reflexivity. - cbn. rewrite -> SuccNat2Pos.id_succ. reflexivity. Qed.
+  Local Notation "'Lextend' f" := (fun ls is => List.FoldResult.fold_left_result0 f is (Success ls)) (at level 0, only parsing).
 
-    Lemma failure_bounds0: forall {T F: Type} {failure: Result.AssertionError F} (ls: list T) (i: Z), @indexing T F ls i failure = Result.assertion_failed <-> (i < 0 \/ (Z.of_nat (length ls)) <= i )%Z.
-    Proof. intros T F [f] ls i. destruct i; delta indexing; cbn beta iota; split; intros.
-      - destruct ls eqn:Eq.
-        + cbn. lia.
-        + easy.
-      - destruct ls.
-        + easy.
-        + destruct H; [ lia | easy ].
-      - destruct (List.nth_error ls (Pos.to_nat p)) eqn:Eq.
-        + easy.
-        + rewrite -> List.nth_error_None in Eq. lia.
-      - destruct H; try lia.
-        rewrite <- positive_nat_Z in H. rewrite <- Nat2Z.inj_le in H.
-        rewrite <- List.nth_error_None in H. rewrite -> H.
-        easy.
-      - lia.
-      - easy.
-    Qed.
+  Module Indexing.
+    Module Nat.
+      Definition indexing {T F: Type} {failure: Result.AssertionError F} (ls: list T) (i: nat): Result.Result T F :=
+        Result.from_option_assertion (List.nth_error ls i).
 
-    Lemma failure_is_assertion: forall {T F: Type} {failure: Result.AssertionError F} (ls: list T) (i: Z) (f: F),
-      indexing ls i = Result.Failure f -> {| Result.f := f |} = failure.
-    Proof.
-      intros T F [f'] ls i f. destruct i; destruct ls; cbn in *; first[ intros [=->] | intros H ]; try easy.
-      - destruct (List.nth_error _ _) eqn:Eq in *.
-        + discriminate.
-        + cbn in *. congruence.
-      - destruct (List.nth_error _ _) eqn:Eq in *.
-        + discriminate.
-        + cbn in *. congruence.
-    Qed.
+      Lemma success_bounds0 {T F: Type} {_: Result.AssertionError F}: forall (ls: list T) (i: nat),
+        (exists v, indexing ls i = Success v) <-> (i < length ls)%nat.
+      Proof.
+        unfold indexing.
+        induction ls; intros i.
+        - split; intros H.
+          + destruct H as [ v H ]. destruct i; Result.assertion_failed_helper.
+          + cbn in H. lia.
+        - destruct i; cbn.
+          + split. * lia. * intros _. exists a. reflexivity.
+          + assert (S i < S (length ls) <-> i < (length ls))%nat as -> by lia.
+            apply IHls.
+      Qed.
+      Lemma success_bounds {T F: Type} {_: Result.AssertionError F}: forall (ls: list T) (i: nat) (v: T),
+        indexing ls i = Success v -> (i < length ls)%nat.
+      Proof. intros. pose proof ((ex_intro (fun v => _ = Success v) v) H) as Bounds_i. rewrite -> success_bounds0 in Bounds_i. assumption. Qed.
 
-    Lemma failure_kind: forall {T F: Type} {failure: Result.AssertionError F} (ls: list T) (i: Z) (f: F),
-      indexing ls i = Result.Failure f -> indexing ls i = Result.assertion_failed.
-    Proof. intros T F f' ls i f H. pose proof (failure_is_assertion ls i f H) as [=]. Result.assertion_failed_helper. Qed.
+      Lemma failure_is_assertion {T F: Type} {f: Result.AssertionError F}: forall (ls: list T) (i: nat) (f': F),
+        indexing ls i = Result.Failure f' -> {| Result.f := f' |} = f.
+      Proof.
+        intros ls i f' Eq_indexed. unfold indexing in *. 
+        destruct (List.nth_error _ _) in *; try discriminate.
+        cbn in Eq_indexed. Result.assertion_failed_helper.
+      Qed.
 
-    Lemma failure_bounds: forall {T F: Type} {failure: Result.AssertionError F} (ls: list T) (i: Z) (f: F), @indexing T F ls i failure = Result.Failure f -> (i < 0 \/ (Z.of_nat (length ls)) <= i )%Z.
-    Proof. intros. pose proof H as H'. apply failure_is_assertion in H. rewrite <- failure_bounds0. Result.assertion_failed_helper. Qed.
+      Lemma failure_kind {T F: Type} {_: Result.AssertionError F}: forall (ls: list T) (i: nat) (f: F),
+        indexing ls i = Result.Failure f -> indexing ls i = Result.assertion_failed.
+      Proof. intros ls i f H. pose proof (failure_is_assertion ls i f H) as [=]. Result.assertion_failed_helper. Qed.
 
-    Lemma success_bounds0: forall {T F: Type} {failure: Result.AssertionError F} (ls: list T) (i: Z),
-      (exists v, indexing ls i = Success v) <-> (0 <= i /\ i < (Z.of_nat (length ls)) )%Z.
-    Proof. intros T F f. split.
-      - intros [ v H ]. pose proof (failure_bounds0 ls i) as [ _ Falsum ].
-        destruct ( (0 <=? i) && (i <? Z.of_nat (length ls)))%Z eqn:Bounds.
-        + Zhelper. lia.
-        + hypotheses_reflector.
-          * rewrite -> Z.leb_gt in H0. specialize (Falsum (or_introl H0)). destruct f. discriminate.
-          * rewrite -> Z.ltb_ge in H0. specialize (Falsum (or_intror H0)). destruct f. discriminate.
-      - intros [ Leq_0_i Le_i_len ]. pose proof (failure_bounds0 ls i) as [ Falsum _ ].
-        destruct i.
-        + destruct ls eqn:Eq_ls; cbn in *; try lia. exists t. reflexivity.
-        + destruct (indexing ls (Z.pos p)) eqn:Eq_indexed in |- *.
-          * exists s. reflexivity.
-          * apply failure_kind in Eq_indexed. specialize (Falsum Eq_indexed).
-            destruct Falsum; lia.
-        + lia.
-    Qed.
+      Lemma failure_bounds0 {T F: Type} {f: Result.AssertionError F}: forall (ls: list T) (i: nat), @indexing T F f ls i = Result.assertion_failed <-> (length ls <= i )%nat.
+      Proof.
+        destruct f as [f]. intros ls i. rewrite <- nth_error_None.
+        unfold indexing.
+        destruct (nth_error ls i) eqn:Eq; cbn in *.
+        - split; discriminate.
+        - split; reflexivity.
+      Qed.
+      Lemma failure_bounds {T F: Type} {f: Result.AssertionError F}: forall (ls: list T) (i: nat) (f': F), @indexing T F f ls i = Result.Failure f' -> (length ls <= i )%nat.
+      Proof. intros. pose proof H as H'. apply failure_is_assertion in H. rewrite <- failure_bounds0. Result.assertion_failed_helper. Qed.
 
-    Lemma success_bounds: forall {T F: Type} {failure: Result.AssertionError F} (ls: list T) (i: Z) (v: T),
-      indexing ls i = Success v -> ( 0 <= i /\ i < (Z.of_nat (length ls)) )%Z.
-    Proof. intros. pose proof ((ex_intro (fun v => _ = Success v) v) H) as Bounds_i. rewrite -> Indexing.success_bounds0 in Bounds_i. assumption. Qed.
+      Lemma nil {T F: Type} {_: Result.AssertionError F}: forall (i: nat),
+        indexing (nil: list T) i = Result.assertion_failed.
+      Proof.
+        intros; destruct i; cbn; try easy.
+      Qed.
 
-    Lemma nil: forall {T F: Type} {failure: Result.AssertionError F} (i: Z),
-      indexing (nil: list T) i = Result.assertion_failed.
-    Proof.
-      intros; destruct i; cbn; try easy.
-      destruct (Pos.to_nat p); reflexivity.
-    Qed.
+      Lemma cons {T F: Type} {_: Result.AssertionError F}: forall (h: T) (t: list T) (i: nat),
+        indexing (h :: t) (S i) = indexing t i.
+      Proof.
+        intros h t i. destruct i.
+        - reflexivity.
+        - destruct t.
+          + reflexivity.
+          + unfold indexing. cbn. reflexivity.
+      Qed.
 
-    Lemma nth_error_cons: forall A h (t: list A) i, nth_error (h :: t) (S i) = nth_error t i.
-    Proof. induction t; intros; reflexivity. Qed.
+      Lemma repeat {T F: Type} {failure: Result.AssertionError F}: forall n v i v',
+        indexing (@List.repeat T v n) i = Success v' -> v = v'.
+      Proof.
+        intros n.
+        induction n.
+        - intros v i v' H. cbn in H. rewrite -> nil in H. Result.assertion_failed_helper.
+        - intros v i v' H. induction i.
+          + injection H as ->. reflexivity.
+          + simpl repeat in H. rewrite -> cons in H.
+            specialize IHn with (1 := H). assumption.
+      Qed.
+    End Nat.
 
-    Lemma cons: forall {T F: Type} {failure: Result.AssertionError F} (h: T) (t: list T) (i: Z),
-      0 <= i -> indexing (h :: t) (i + 1) = indexing t i.
-    Proof.
-      intros; destruct t; destruct (i + 1) eqn:Eq_Si; try lia.
-      - cbn. destruct (Pos.to_nat p) eqn:Eq_p; try lia. cbn. rewrite -> nil. destruct n; reflexivity.
-      - cbn. pose proof (Pos2Nat.is_succ p) as [i' Eq_i']. rewrite -> Eq_i'.
-        assert (i = Z.of_nat i') as Eq_ii' by lia.
-        rewrite -> Eq_ii' in *. subst. clear Eq_i'. clear Eq_Si. clear p.
-        rename i' into i.
-        destruct i eqn:Eq_i.
-        + reflexivity.
-        + cbn. rewrite -> SuccNat2Pos.id_succ. rewrite -> nth_error_cons. reflexivity.
-    Qed.
+    Module Int.
+      Definition indexing {T F: Type} {_: Result.AssertionError F}: list T -> Z -> Result.Result T F := Zextend Nat.indexing.
+
+      Lemma success_bounds0 {T F: Type} {_: Result.AssertionError F}: forall (ls: list T) (i: Z),
+        (exists v, indexing ls i = Success v) <-> (0 <= i /\ i < Z.of_nat (length ls))%Z.
+      Proof.
+        unfold indexing. intros ls i. destruct i.
+        - assert ((0 <= 0 < Z.of_nat (length ls))%Z <-> (0 < length ls)%nat) as -> by lia. apply Nat.success_bounds0.
+        - assert ((0 <= Z.pos p < Z.of_nat (length ls))%Z <-> (Pos.to_nat p < length ls)%nat) as -> by lia. apply Nat.success_bounds0.
+        - split. + intros [ v Falsum ]. Result.assertion_failed_helper. + lia.
+      Qed.
+      Lemma success_bounds {T F: Type} {_: Result.AssertionError F}: forall (ls: list T) (i: Z) (v: T),
+        indexing ls i = Success v -> (0 <= i /\ i < Z.of_nat (length ls))%Z.
+      Proof. intros. pose proof ((ex_intro (fun v => _ = Success v) v) H) as Bounds_i. rewrite -> success_bounds0 in Bounds_i. assumption. Qed.
+
+      Lemma failure_is_assertion {T F: Type} {f: Result.AssertionError F}: forall (ls: list T) (i: Z) (f': F),
+          indexing ls i = Result.Failure f' -> {| Result.f := f' |} = f.
+      Proof.
+        unfold indexing. intros ls i f' Eq_indexed. destruct i.
+        - apply Nat.failure_is_assertion in Eq_indexed. assumption.
+        - apply Nat.failure_is_assertion in Eq_indexed. assumption.
+        - Result.assertion_failed_helper.
+      Qed.
+
+      Lemma failure_kind {T F: Type} {_: Result.AssertionError F}: forall (ls: list T) (i: Z) (f: F),
+        indexing ls i = Result.Failure f -> indexing ls i = Result.assertion_failed.
+      Proof. intros ls i f H. pose proof (failure_is_assertion ls i f H) as [=]. Result.assertion_failed_helper. Qed.
+
+      Lemma failure_bounds0 {T F: Type} {f: Result.AssertionError F}: forall (ls: list T) (i: Z), @indexing T F f ls i = Result.assertion_failed <-> (i < 0 \/ (Z.of_nat (length ls)) <= i )%Z.
+      Proof.
+        unfold indexing. intros ls i. destruct i.
+        - rewrite -> Nat.failure_bounds0. lia.
+        - rewrite -> Nat.failure_bounds0. lia.
+        - cbn. split. + lia. + reflexivity.
+      Qed.
+
+      Lemma failure_bounds {T F: Type} {f: Result.AssertionError F}: forall (ls: list T) (i: Z) (f': F), @indexing T F f ls i = Result.Failure f' -> (i < 0 \/ (Z.of_nat (length ls)) <= i )%Z.
+      Proof. intros. pose proof H as H'. apply failure_is_assertion in H. rewrite <- failure_bounds0. Result.assertion_failed_helper. Qed.
+
+      Lemma nil: forall {T F: Type} {f: Result.AssertionError F} (i: Z),
+        indexing (nil: list T) i = Result.assertion_failed.
+      Proof.
+        intros; destruct i; cbn; try easy.
+        destruct (Pos.to_nat p); reflexivity.
+      Qed.
+
+      Lemma cons {T F: Type} {_: Result.AssertionError F}: forall (h: T) (t: list T) (i: Z),
+        (0 <= i) -> indexing (h :: t) (i + 1) = indexing t i.
+      Proof.
+        unfold indexing.
+        intros h t i Ineq_0_i. destruct i; cbn.
+        - apply Nat.cons.
+        - assert (Pos.to_nat (p + 1) = S (Pos.to_nat p)) as -> by lia. apply Nat.cons.
+        - lia.
+      Qed.
+      
+      Lemma repeat {T F: Type} {failure: Result.AssertionError F}: forall n v i v',
+        indexing (@List.repeat T v n) i = Success v' -> v = v'.
+      Proof. intros n v i v' H. destruct i. - apply Nat.repeat with (1 := H). - apply Nat.repeat with (1 := H). - apply Indexing.Int.success_bounds in H. lia. Qed.
+      
+      (** Int only theorems *)
+
+      Lemma of_nat {T F: Type} {failure: Result.AssertionError F}: forall (ls: list T) (i: nat), indexing ls (Z.of_nat i) = Nat.indexing ls i.
+      Proof. intros. destruct i. - reflexivity. - cbn. rewrite -> SuccNat2Pos.id_succ. reflexivity. Qed.
+
+      Lemma to_nat {T F: Type} {failure: Result.AssertionError F}: forall (ls: list T) (i: Z), (0 <= i)%Z -> indexing ls i = Nat.indexing ls (Z.to_nat i).
+      Proof. intros. destruct i. - reflexivity. - reflexivity. - lia. Qed.
+
+      Lemma cons_of_nat {T F: Type} {_: Result.AssertionError F}: forall (h: T) (t: list T) (i: nat) (v: T),
+        indexing (h :: t) (Z.of_nat (S i)) = Success v <-> indexing t (Z.of_nat i) = Success v.
+      Proof.
+        intros. assert (Z.of_nat (S i) = Z.of_nat i + 1) as -> by lia.
+        split; intros H.
+        - rewrite -> cons in H by lia. assumption.
+        - rewrite -> cons by lia. assumption.
+      Qed.
+    End Int.
   End Indexing.
 
-  Module Updating.
-    Fixpoint updating_nat {T F: Type} (ls: list T) (i: nat) (v: T) {failure: Result.AssertionError F}: Result.Result (list T) F := match ls with
-    | nil => Result.assertion_failed
-    | h :: t =>  match i with
-      | 0%nat => Success (v :: t)
-      | S i' => let! t' =<< updating_nat t i' v in Success (h :: t')
-      end
-    end.
+  Module Forall.
+    Definition Forall {T F: Type} {_: Result.AssertionError F} (ls: list T) (P: T -> Prop) := (forall i v, Indexing.Nat.indexing ls i = Success v -> P v).
 
+    Lemma nil {T F: Type} {_: Result.AssertionError F}: forall (P: T -> Prop), Forall nil P.
+    Proof. intros P i v H. apply Indexing.Nat.success_bounds in H. cbn in H. lia. Qed.
+
+    Lemma cons {T F: Type} {_: Result.AssertionError F}: forall (h: T) (t: list T) (P: T -> Prop), P h -> Forall t P -> Forall (h :: t) P.
+    Proof.
+      intros h t P Hh Ht i v Eq_indexed. destruct i.
+      - injection Eq_indexed as <-. assumption.
+      - rewrite -> Indexing.Nat.cons in Eq_indexed. apply (Ht i v Eq_indexed).
+    Qed.
+
+    Lemma cons_inv_head {T F: Type} {_: Result.AssertionError F}: forall (h: T) (t: list T) (P: T -> Prop), Forall (h :: t) P -> P h.
+    Proof. intros h t P F_h_t. specialize (F_h_t 0%nat h). cbn in *. fforward. assumption. Qed.
+
+    Lemma cons_inv_tail {T F: Type} {_: Result.AssertionError F}: forall (h: T) (t: list T) (P: T -> Prop), Forall (h :: t) P -> Forall t P.
+    Proof. intros h t P F_h_t i v Eq_indexed. specialize (F_h_t (S i) v). apply F_h_t. rewrite -> Indexing.Nat.cons. assumption. Qed.
+
+    Lemma cons_inv {T F: Type} {_: Result.AssertionError F}: forall (h: T) (t: list T) (P: T -> Prop), Forall (h :: t) P -> P h /\ Forall t P.
+    Proof. intros h t P F_h_t. split. - eapply cons_inv_head; eassumption. - eapply cons_inv_tail; eassumption. Qed.
+
+    Lemma concat {T F: Type} {_: Result.AssertionError F}: forall (ls ls': list T) (P: T -> Prop), Forall ls P -> Forall ls' P -> Forall (ls ++ ls') P.
+    Proof.
+      induction ls; intros ls' P F_ls F_ls'; cbn.
+      - assumption.
+      - apply cons_inv in F_ls as [ P_a F_ls ]. intros [ | i ] v Eq_indexed.
+        + cbn in Eq_indexed. injection Eq_indexed as <-. assumption.
+        + rewrite -> Indexing.Nat.cons in Eq_indexed. specialize IHls with (1 := F_ls) (2 := F_ls'). specialize (IHls _ _ Eq_indexed). assumption.
+    Qed.
+
+    Lemma repeat {T F: Type} {_: Result.AssertionError F}: forall (n: nat) (t: T) (P: T -> Prop), P t -> Forall (List.repeat t n) P.
+    Proof. intros n t P H i v Eq_indexed. apply Indexing.Nat.repeat in Eq_indexed. subst. assumption. Qed.
+
+    Lemma to_Z {T F: Type} {_: Result.AssertionError F}: forall (ls: list T) (P: T -> Prop), Forall ls P -> forall i v, Indexing.Int.indexing ls i = Success v -> P v.
+    Proof.
+      intros ls P H [ | z | z ] v Eq_indexed.
+      - rewrite -> Indexing.Int.to_nat in Eq_indexed by lia.
+        cbn in Eq_indexed.
+        apply (H _ _ Eq_indexed).
+      - rewrite -> Indexing.Int.to_nat in Eq_indexed by lia.
+        cbn in Eq_indexed.
+        apply (H _ _ Eq_indexed).
+      - apply Indexing.Int.success_bounds in Eq_indexed. lia.
+    Qed.
+  End Forall.
+
+  Module Update.
+    Module Nat.
+      Module One.
+        Fixpoint update {T F: Type} {_: Result.AssertionError F} (v: T) (ls: list T) (i: nat): Result.Result (list T) F := match ls with
+          | nil => Result.assertion_failed
+          | h :: t =>  match i with
+            | 0%nat => Success (v :: t)
+            | S i' => let! t' =<< update v t i' in Success (h :: t')
+            end
+          end.
+
+        Lemma cons_inv_tail {T F: Type} {_: Result.AssertionError F}: forall (h: T) (t: list T) (i: nat) (v: T),
+          update v (h :: t) (S i) = (let! t' =<< update v t i in Success (h :: t')).
+        Proof. intros h t i v. cbn. destruct (update v t i); reflexivity. Qed.
+
+        Lemma failure_is_assertion {T F: Type} {f: Result.AssertionError F}: forall (ls: list T) (i: nat) (v: T) (f': F),
+          update v ls i = Result.Failure f' -> {| Result.f := f' |} = f.
+        Proof.
+          induction ls; intros i v f'.
+          - cbn. Result.assertion_failed_helper. intros [=<-]. reflexivity.
+          - destruct i.
+            + discriminate.
+            + intros H. cbn in H. destruct (update v ls i) eqn:Eq_update; try discriminate.
+              injection H as <-. apply IHls with (i := i) (v := v). assumption.
+        Qed.
+
+        Lemma failure_kind {T F: Type} {_: Result.AssertionError F}: forall (ls: list T) (i: nat) (v: T) (f: F),
+          update v ls i = Result.Failure f -> update v ls i = Result.assertion_failed.
+        Proof. intros ls i v f H. pose proof (failure_is_assertion ls i v f H) as [=]. Result.assertion_failed_helper. Qed.
+
+        Lemma failure_bounds0 {T F: Type} {f: Result.AssertionError F}: forall (ls: list T) (i: nat) (v: T),
+          @update T F f v ls i = Result.assertion_failed <-> (length ls <= i)%nat.
+        Proof.
+        Admitted.
+
+        Lemma failure_bounds {T F: Type} {f: Result.AssertionError F}: forall (ls: list T) (i: nat) (v: T) (f': F),
+          @update T F f v ls i = Result.Failure f' -> (length ls <= i)%nat.
+        Proof. intros. pose proof H as H'. apply failure_is_assertion in H. rewrite <- failure_bounds0 with (v := v). Result.assertion_failed_helper. Qed.
+
+        Lemma success_length {T F: Type} {_: Result.AssertionError F}: forall (ls ls': list T) (i: nat) (v: T),
+          update v ls i = Success ls' -> (length ls) = (length ls').
+        Proof.
+          intros ls. induction ls; intros ls' i v H.
+          - Result.assertion_failed_helper.
+          - destruct i.
+            + injection H as <-. reflexivity.
+            + cbn in *. destruct (update v ls i) eqn:Eq_updated; try discriminate.
+              injection H as <-. cbn. f_equal.
+              apply IHls with (1 := Eq_updated).
+        Qed.
+
+        Lemma indexing_updated_same {T F: Type} {_: Result.AssertionError F}: forall i (ls: list T) v ls',
+          update v ls i = Success ls' -> Indexing.Nat.indexing ls' i = Success v.
+        Proof.
+          induction i; intros ls v ls' H; destruct ls; cbn in *; Result.assertion_failed_helper.
+          - injection H as <-. reflexivity.
+          - destruct (update v ls i) eqn:Eq_indexed; try discriminate.
+            injection H as <-.
+            specialize IHi with (1 := Eq_indexed) as <-.
+            apply Indexing.Nat.cons.
+        Qed.
+
+       Lemma indexing_updated_other {T F: Type} {_: Result.AssertionError F}: forall i (ls: list T) v ls',
+          update v ls i = Success ls' -> forall j, i <> j -> Indexing.Nat.indexing ls' j = Indexing.Nat.indexing ls j.
+        Proof.
+          induction i; intros ls v ls' H j Neq_i_j; destruct ls; cbn in *; Result.assertion_failed_helper.
+          - injection H as <-. destruct j; try lia. reflexivity.
+          - destruct (update v ls i) eqn:Eq_updated; try discriminate.
+            injection H as <-.
+            destruct j.
+            + reflexivity.
+            + repeat rewrite -> Indexing.Nat.cons.
+              apply IHi with (1 := Eq_updated). lia.
+        Qed.
+
+        Lemma prop_preservation {T F: Type} {_: Result.AssertionError F}: forall (ls: list T) i v ls' P,
+          Forall.Forall ls P ->
+          P v ->
+          update v ls i = Success ls' ->
+          Forall.Forall ls' P.
+        Proof.
+          intros ls i v ls' P H Pv Eq_ls' j w Eq_indexed.
+          destruct (Nat.eq_dec i j) as [ <- | Neq_i_j ].
+          - apply indexing_updated_same in Eq_ls'.
+            rewrite Eq_ls' in Eq_indexed. injection Eq_indexed as ->.
+            assumption.
+          - apply H with (i := j).
+            rewrite <- Eq_indexed. symmetry.
+            rewrite -> indexing_updated_other with (1 := Eq_ls') (2 := Neq_i_j).
+            reflexivity.
+        Qed.
+      End One.
+
+      Module Batch.
+        Definition update {T F: Type} {_: Result.AssertionError F} (v: T) := Lextend (One.update v).
+
+        Lemma step {T F: Type} {_: Result.AssertionError F}: forall (ls: list T) (i: nat) (is: list nat) (v: T),
+          update v ls (i :: is) = let! ls' =<< One.update v ls i in update v ls' is.
+        Proof. intros ls i is v. cbn. destruct is; cbn in *. - focus § _ _ [] § auto destruct; reflexivity. - reflexivity. Qed.
+
+        Lemma failure_is_assertion {T F: Type} {f: Result.AssertionError F}: forall (is: list nat) (ls: list T) (v: T) (f': F),
+          update v ls is = Result.Failure f' -> {| Result.f := f' |} = f.
+        Proof.
+          induction is; intros ls v f' H.
+          - discriminate.
+          - rewrite -> step in H. destruct (One.update v ls a) eqn:Eq_update.
+            + apply IHis with (ls := s) (v := v). assumption.
+            + apply One.failure_is_assertion in Eq_update. congruence.
+        Qed.
+
+        Lemma failure_bounds {T F: Type} {f: Result.AssertionError F}: forall (is: list nat) (ls: list T) (v: T) (f': F),
+          @update T F f v ls is = Result.Failure f' -> ~ Forall.Forall is (fun i => i < length ls)%nat.
+        Proof.
+          induction is; intros; intros Falsum.
+          - discriminate.
+          - cbn in H. destruct (One.update v ls a) eqn:Eq_update.
+            + specialize IHis with (1 := H). apply Forall.cons_inv_tail in Falsum. apply IHis. intros j w G. apply One.success_length in Eq_update as <-.
+              specialize (Falsum j w). fforward. apply Falsum.
+            + apply One.failure_bounds in Eq_update. specialize (Falsum 0%nat a). cbn in Falsum. fforward. lia.
+        Qed.
+
+        Lemma success_length {T F: Type} {_: Result.AssertionError F}: forall (is: list nat) (ls ls': list T) (v: T),
+          update v ls is = Success ls' -> (length ls) = (length ls').
+        Proof.
+          induction is; intros ls0 ls2 v H; cbn in H.
+          - injection H as <-. reflexivity.
+          - destruct (One.update v ls0 a) as [ ls1 | ] eqn:Eq_ls1.
+            + apply One.success_length in Eq_ls1 as ->.
+              apply IHis with (v := v). apply H.
+            + rewrite -> FoldResult.zero_failure0 in H. discriminate.
+        Qed.
+
+        Lemma prop_preservation {T F: Type} {_: Result.AssertionError F}: forall is (ls: list T) v ls' P,
+          Forall.Forall ls P ->
+          P v ->
+          update v ls is = Success ls' ->
+          Forall.Forall ls' P.
+        Proof.
+          induction is; intros ls v ls' P FP_ls P_v Eq_ls'.
+          - cbn in Eq_ls'. injection Eq_ls' as <-. assumption.
+          - cbn in Eq_ls'.
+            destruct (One.update v ls a) eqn:Eq_update.
+            + apply IHis with (ls := s) (v := v); try assumption.
+              apply One.prop_preservation with (ls := ls) (i := a) (v := v); try assumption.
+            + rewrite FoldResult.zero_failure0 in Eq_ls'. discriminate.
+        Qed.
+
+      End Batch.
+    End Nat.
+(* 
     Definition updating {T F: Type} (ls: list T) (i: Z) (v: T) {failure: Result.AssertionError F}: Result.Result (list T) F := match i with
     | Z0 => updating_nat ls 0 v
     | Zpos i => updating_nat ls (Pos.to_nat i) v
     | Zneg _ => Result.assertion_failed
     end.
+
+    Definition batch_updating0_nat {T F: Type} {_: Result.AssertionError F} (ls: Result (list T) F) (is: list nat) (v: T) := List.FoldResult.fold_left_result0 (fun ls i => List.Updating.updating_nat ls i v) is ls.
+    Definition batch_updating_nat {T F: Type} {_: Result.AssertionError F} (ls: list T) (is: list nat) (v: T) := List.FoldResult.fold_left_result (fun ls i => List.Updating.updating_nat ls i v) is ls.
+
+    Definition batch_updating0 {T F: Type} {_: Result.AssertionError F} (ls: Result (list T) F) (is: list Z) (v: T) := List.FoldResult.fold_left_result0 (fun ls i => List.Updating.updating ls i v) is ls.
+    Definition batch_updating {T F: Type} {_: Result.AssertionError F} (ls: list T) (is: list Z) (v: T) := List.FoldResult.fold_left_result (fun ls i => List.Updating.updating ls i v) is ls.
+
+    Lemma batch_nat_cons {T F: Type} {_: Result.AssertionError F}: forall (ls: list T) (i: nat) (is: list nat) (v: T),
+      batch_updating_nat ls (i :: is) v = let! ls' =<< updating_nat ls i v in batch_updating_nat ls' is v.
+    Proof. intros ls i is v. unfold batch_updating_nat. rewrite -> FoldResult.cons. reflexivity. Qed.
+    Lemma batch_cons {T F: Type} {_: Result.AssertionError F}: forall (ls: list T) (i: Z) (is: list Z) (v: T),
+      batch_updating ls (i :: is) v = let! ls' =<< updating ls i v in batch_updating ls' is v.
+    Proof. intros ls i is v. unfold batch_updating. rewrite -> FoldResult.cons. reflexivity. Qed.
+
+    Lemma success_length_nat {T F: Type} {f: Result.AssertionError F}: forall (ls ls': list T) (i: nat) (v: T), updating_nat ls i v = Success ls' -> (length ls) = (length ls').
+    Proof.
+      intros ls. induction ls; intros ls' i v H.
+      - Result.assertion_failed_helper.
+      - destruct i.
+        + injection H as <-. reflexivity.
+        + cbn in *. destruct (updating_nat ls i v) eqn:Eq_updated; try discriminate.
+          injection H as <-. cbn. f_equal.
+          apply IHls with (1 := Eq_updated).
+    Qed.
+
+    Lemma success_length {T F: Type} {f: Result.AssertionError F}: forall (ls ls': list T) (i: Z) (v: T), updating ls i v = Success ls' -> (length ls) = (length ls').
+    Proof. intros ls ls' i v H. induction i using pseudo_nat_ind. - apply success_length_nat with (1 := H). - apply success_length_nat with (1 := H). - Result.assertion_failed_helper. Qed.
+
+    Lemma of_nat {T F: Type} {f: Result.AssertionError F}: forall (ls: list T) (i: nat) (v: T), updating_nat ls i v = updating ls (Z.of_nat i) v.
+    Proof. intros. destruct i; cbn; try rewrite -> SuccNat2Pos.id_succ; reflexivity. Qed.
 
     Lemma failure_bounds_nat: forall {T F: Type} {failure: Result.AssertionError F} (ls: list T) (i: nat) (v: T), @updating_nat T F ls i v failure = Result.assertion_failed <-> (length ls <= i )%nat.
     Proof. 
@@ -166,6 +469,10 @@ Module List.
       updating_nat ls i v = Result.Failure f -> updating_nat ls i v = Result.assertion_failed.
     Proof. intros. pose proof (failure_is_assertion_nat ls i f v H). Result.assertion_failed_helper. Qed.
 
+(*     Lemma failure_kind {T F: Type} {failure: Result.AssertionError F}: forall (ls: list T) (i: Z) (f: F) (v: T),
+      updating ls i v = Result.Failure f -> updating ls i v = Result.assertion_failed.
+    Proof. intros ls i f v H. destruct i. - apply failure_kind_nat with (f := f). apply H. - apply failure_kind_nat with (f := f). apply H. - Result.assertion_failed_helper. Qed.
+ *)
     Lemma failure_bounds: forall {T F: Type} {failure: Result.AssertionError F} (ls: list T) (i: Z) (v: T), @updating T F ls i v failure = Result.assertion_failed <-> (i < 0 \/ Z.of_nat (length ls) <= i )%Z.
     Proof.
       intros. split.
@@ -182,6 +489,52 @@ Module List.
         + lia.
     Qed.
 
+    Lemma batch_failure_bounds {T F: Type} {f: Result.AssertionError F}: forall (is: list Z) (ls: list T) (v: T),
+      @batch_updating T F f ls is v = Result.assertion_failed
+      ->
+      (exists j i, Indexing.indexing is j = Success i /\ (i < 0 \/ Z.of_nat (length ls) <= i) )%Z.
+    Proof.
+      assert (forall (is: list Z) (ls: list T) (v: T),
+        @batch_updating T F f ls is v = Result.assertion_failed
+        ->
+        (exists j i, Indexing.indexing is j = Success i /\ (i < 0 \/ Z.of_nat (length ls) <= i) )%Z
+      ) as LtR. {
+        induction is; intros ls v Eq_failure.
+        - Result.assertion_failed_helper.
+        - rewrite batch_cons in Eq_failure.
+          destruct (updating ls a v) eqn:Eq_updated.
+          + apply IHis in Eq_failure. destruct Eq_failure as [ j [ i [ Eq_indexed Ineq_i ]]].
+            pose proof (Indexing.success_bounds _ _ _ Eq_indexed) as B_j.
+            exists (j + 1). exists i.
+            split. * rewrite -> Indexing.cons0; [ apply Eq_indexed | lia ]. * apply Updating.success_length in Eq_updated. lia.
+          + exists 0. exists a. split. * reflexivity. * rewrite <- failure_bounds with (v := v). Result.assertion_failed_helper.
+      }
+      apply LtR.
+    Qed.
+    
+    Lemma batch_nat_failure_bounds {T F: Type} {f: Result.AssertionError F}: forall (is: list nat) (ls: list T) (v: T),
+      @batch_updating_nat T F f ls is v = Result.assertion_failed
+      ->
+      (exists j i, Indexing.indexing is j = Success i /\ (length ls <= i))%nat.
+    Proof.
+      assert (forall (is: list nat) (ls: list T) (v: T),
+        @batch_updating_nat T F f ls is v = Result.assertion_failed
+        ->
+        (exists j i, Indexing.indexing is j = Success i /\ (length ls <= i) )%nat
+      ) as LtR. {
+        induction is; intros ls v Eq_failure.
+        - Result.assertion_failed_helper.
+        - rewrite batch_nat_cons in Eq_failure.
+          destruct (updating_nat ls a v) eqn:Eq_updated.
+          + apply IHis in Eq_failure. destruct Eq_failure as [ j [ i [ Eq_indexed Ineq_i ]]].
+            pose proof (Indexing.success_bounds _ _ _ Eq_indexed) as B_j.
+            exists (j + 1). exists i.
+            split. * rewrite -> Indexing.cons0; [ apply Eq_indexed | lia ]. * apply Updating.success_length_nat in Eq_updated. lia.
+          + exists 0. exists a. split. * reflexivity. * rewrite <- failure_bounds_nat with (v := v). Result.assertion_failed_helper.
+      }
+      apply LtR.
+    Qed.
+
     Lemma failure_is_assertion: forall {T F: Type} {failure: Result.AssertionError F} (ls: list T) (i: Z) (f: F) (v: T),
       updating ls i v = Result.Failure f -> {| Result.f := f |} = failure.
     Proof.
@@ -195,6 +548,18 @@ Module List.
       updating ls i v = Result.Failure f -> updating ls i v = Result.assertion_failed.
     Proof. intros. pose proof (failure_is_assertion ls i f v H). Result.assertion_failed_helper. Qed.
 
+    Lemma batch_failure_kind: forall {T F: Type} {failure: Result.AssertionError F} (is: list Z) (ls: list T) (f: F) (v: T),
+      batch_updating ls is v = Result.Failure f -> batch_updating ls is v = Result.assertion_failed.
+    Proof.
+      induction is; intros ls f v H.
+      - Result.assertion_failed_helper.
+      - rewrite -> batch_cons.
+        destruct (updating ls a v) eqn:Eq_updated.
+        * rewrite -> Updating.batch_cons in H. rewrite -> Eq_updated in H. apply IHis with (1 := H).
+        * pose proof (failure_kind _ _ _ _ Eq_updated) as Tmp. Result.assertion_failed_helper. rewrite -> Eq_updated in Tmp. injection Tmp as ->.
+          reflexivity.
+    Qed.
+
     Lemma success_bounds: forall {T F: Type} {failure: Result.AssertionError F} (ls: list T) (i: Z) (v: T),
       (exists ls', updating ls i v = Success ls') <-> (0 <= i /\ i < (Z.of_nat (length ls)) )%Z.
     Proof. intros T F f. split.
@@ -202,8 +567,8 @@ Module List.
         destruct ( (0 <=? i) && (i <? Z.of_nat (length ls)))%Z eqn:Bounds.
         + Zhelper. lia.
         + hypotheses_reflector.
-          * rewrite -> Z.leb_gt in H0. specialize (Falsum (or_introl H0)). destruct f. discriminate.
-          * rewrite -> Z.ltb_ge in H0. specialize (Falsum (or_intror H0)). destruct f. discriminate.
+          * rewrite -> Z.leb_gt in H0. specialize (Falsum (or_introl H0)). destruct f. rewrite -> H in *. discriminate.
+          * rewrite -> Z.ltb_ge in H0. specialize (Falsum (or_intror H0)). destruct f. rewrite -> H in *. discriminate.
       - intros [ Leq_0_i Le_i_len ]. pose proof (failure_bounds ls i v) as [ Falsum _ ].
         destruct i eqn:Eq_i.
         + destruct ls eqn:Eq_ls; cbn in *; try lia. exists (v :: l). reflexivity.
@@ -213,13 +578,137 @@ Module List.
             destruct Falsum; lia.
         + lia.
     Qed.
-  End Updating.
+
+    Lemma nil {T F: Type} {failure: Result.AssertionError F}: forall (i: Z) (v: T), updating nil i v = Result.assertion_failed.
+    Proof. intros. destruct i; reflexivity. Qed.
+
+    Lemma cons_nat {T F: Type} {failure: Result.AssertionError F}: forall (t: list T) (h: T) (i: nat) (v: T),
+      updating_nat (h :: t) (S i) v = (let! t' =<< updating_nat t i v in Success (h :: t')).
+    Proof.
+      induction t; intros h i v.
+      - reflexivity.
+      - destruct i eqn:Eq_i.
+        + reflexivity.
+        + rewrite -> IHt. reflexivity.
+    Qed.
+
+    Lemma cons {T F: Type} {failure: Result.AssertionError F}: forall (h: T) (t: list T) (i: Z) (v: T),
+      0 <= i -> updating (h :: t) (i + 1) v = (let! t' =<< updating t i v in Success (h :: t')).
+    Proof.
+      intros h t i v Ineq_i.
+      destruct i eqn:Eq_i; cbn -[updating_nat].
+      - assert (Pos.to_nat 1 = 1%nat) as -> by lia.
+        rewrite -> cons_nat. reflexivity.
+      - assert (Pos.to_nat (p + 1) = S (Pos.to_nat p)) as -> by lia.
+        rewrite -> cons_nat. reflexivity.
+      - lia.
+    Qed.
+
+    Lemma cons_of_nat {T F: Type} {failure: Result.AssertionError F}: forall (h: T) (t: list T) (i: nat) (v: T),
+      updating (h :: t) (Z.of_nat (S i)) v = (let! t' =<< updating t (Z.of_nat i) v in Success (h :: t')).
+    Proof. intros h t i v. assert (Z.of_nat (S i) = Z.of_nat i + 1) as -> by lia. apply cons. lia. Qed.
+
+    Lemma indexing_updated_same {T F: Type} {failure: Result.AssertionError F}: forall i (ls: list T) v ls',
+      updating ls i v = Success ls' -> Indexing.indexing ls' i = Success v.
+    Proof.
+      induction i using pseudo_nat_ind; intros ls v ls' H; (destruct ls; [ Result.assertion_failed_helper | ]).
+      - injection H as [=<-]. reflexivity.
+      - cbn in H. rewrite -> SuccNat2Pos.id_succ in H.
+        focus § _ [] _ § auto destruct in H.
+        injection H as [=<-].
+        rewrite -> Indexing.cons_of_nat_succ.
+        apply IHi with (ls := ls).
+        rewrite <- Updating.of_nat. assumption.
+      - Result.assertion_failed_helper.
+    Qed.
+
+    Lemma indexing_updated_other {T F: Type} {failure: Result.AssertionError F}: forall i (ls: list T) v ls',
+      updating ls i v = Success ls' -> forall j, i <> j -> Indexing.indexing ls' j = Indexing.indexing ls j.
+    Proof.
+      induction i using pseudo_nat_ind; intros ls v ls' H j Ineq_j; (destruct ls; [ solve[ Result.assertion_failed_helper ] | ]).
+      - injection H as [=<-]. induction j using pseudo_nat_ind.
+        + lia.
+        + focus § _ _ [] § do (fun t => destruct t eqn:Eq_indexed).
+          * rewrite -> Indexing.cons_of_nat_succ in *. assumption.
+          * replace (Z.of_nat (S n)) with ((Z.of_nat n) + 1) in * by lia.
+            rewrite -> Indexing.cons0 in * by lia.
+            assumption.
+        + cbn. reflexivity.
+      - rewrite -> cons_of_nat in H. focus § _ [] _ § auto destruct in H.
+        injection H as <-.
+        destruct j; try reflexivity.
+        assert (Z.pos p = (Z.pos p - 1) + 1) as -> by lia.
+        do 2 rewrite -> Indexing.cons0 by lia.
+        apply IHi with (v := v).
+        + assumption.
+        + lia.
+      - Result.assertion_failed_helper.
+    Qed.
+
+    Lemma prop_preservation {T F: Type} {failure: Result.AssertionError F}: forall (ls: list T) i v ls' P,
+      Forall ls P ->
+      P v ->
+      updating ls i v = Success ls' ->
+      Forall ls' P.
+    Proof.
+      intros ls i v ls' P H Pv Eq_ls' j w Eq_indexed.
+      destruct (Z.eq_dec i j) as [ Eq_ij | Neq_ij ].
+      - subst. apply indexing_updated_same in Eq_ls'.
+        rewrite Eq_ls' in *. injection Eq_indexed as ->.
+        assumption.
+      - apply H with (i := j).
+        rewrite <- Eq_indexed. symmetry.
+        apply indexing_updated_other with (1 := Eq_ls') (2 := Neq_ij).
+    Qed.
+    
+
+    Lemma batch_equiv {T F: Type} {_: Result.AssertionError F}: forall ls is v,
+      @batch_updating0 T F _ (Success ls) is v = @batch_updating T F _ ls is v.
+    Proof. reflexivity. Qed.
+
+    Lemma batch_prop_preservation {T F: Type} {failure: Result.AssertionError F}: forall is (ls: list T) v ls' P,
+      Forall ls P ->
+      P v ->
+      batch_updating ls is v = Success ls' ->
+      Forall ls' P.
+    Proof.
+      induction is; intros ls v ls' P FP_ls P_v Eq_ls'.
+      - cbn in Eq_ls'. injection Eq_ls' as <-. assumption.
+      - cbn in Eq_ls'.
+        focus § _ [] _ § replace with (batch_updating0 (updating ls a v) is v) in Eq_ls'.
+        destruct (updating ls a v) eqn:Eq_updated.
+        + apply IHis with (2 := P_v) (3 := Eq_ls').
+          intros i w Eq_indexed.
+          destruct (Z.eq_dec a i) as [ Eq_ai | Neq_ai ].
+          * subst. pose proof (indexing_updated_same _ _ _ _ Eq_updated).
+            assert (v = w) as -> by congruence. assumption.
+          * pose proof (indexing_updated_other _ _ _ _ Eq_updated _ Neq_ai).
+            apply (FP_ls i w). congruence.
+        + pose proof (FoldResult.zero_failure0 (fun ls i => updating ls i v) is f).
+          unfold batch_updating0 in Eq_ls'. congruence.
+    Qed.
+  End Updating. *)
+  End Update.
 
   Module Exists.
     Fixpoint exist {T F: Type} (ls: list T) (p: T -> Result bool F): Result bool F := match ls with
     | nil => Success false
     | h :: t => let! b: bool =<< p h in if b then Success true else exist t p
     end.
+
+    Lemma failure_kind {T F: Type} {_: Result.AssertionError F}: forall ls p f,
+      @exist T F ls p = Failure f -> exists i v, Indexing.Int.indexing ls i = Success v /\ p v = Failure f.
+    Proof.
+      induction ls; intros p f Ex; try discriminate.
+      cbn in Ex. destruct (p a) as [ [ | ] | ] eqn:Eq.
+      - discriminate.
+      - specialize IHls with (1 := Ex). destruct IHls as [ i [ v [ Indexed ]]].
+        exists (i+1). exists v.
+        rewrite -> Indexing.Int.cons.
+        + split; assumption.
+        + apply Indexing.Int.success_bounds in Indexed. destruct Indexed as [ Indexed _ ]. apply Indexed.
+      - injection Ex as ->. exists 0. exists a. cbn. split; [ reflexivity | assumption].
+    Qed.
   End Exists.
 
   Module Range.
@@ -233,7 +722,7 @@ Module List.
       Proof. induction l; intros b; cbn. - reflexivity. - rewrite -> IHl. reflexivity. Qed.
 
       Lemma indexing {F: Type} {f: Result.AssertionError F}: forall i b l v,
-        Indexing.indexing (range b l) i = Success v -> v = (b + i).
+        Indexing.Int.indexing (range b l) i = Success v -> v = (b + i).
       Proof.
         induction i using pseudo_nat_ind.
         - intros. cbn in *.
@@ -242,14 +731,14 @@ Module List.
         - intros. cbn in *. rewrite -> SuccNat2Pos.id_succ in H.
           destruct l; try Result.assertion_failed_helper. cbn in *.
           specialize (IHi (b + 1) l). cbn in IHi.
-          rewrite -> Indexing.of_nat in *. specialize (IHi _ H).
+          rewrite -> Indexing.Int.of_nat in *. specialize (IHi _ H).
           lia.
         - intros. cbn in H. Result.assertion_failed_helper.
       Qed.
     End Impl.
 
     Definition IsRange (from to: Z) (ls: list Z) :=
-      (forall (F: Type) (f: Result.AssertionError F) z, from <= z < to -> Indexing.indexing ls (z - from) = Success z).
+      (forall (F: Type) (f: Result.AssertionError F) z, from <= z < to -> Indexing.Int.indexing ls (z - from) = Success z).
 
     Definition range(from to: Z) := Impl.range from (Z.to_nat (to - from)).
 
@@ -257,24 +746,24 @@ Module List.
     Proof. unfold range. intros. apply Impl.length. Qed.
 
     Lemma indexing {F: Type} {f: Result.AssertionError F}: forall s e i v,
-      Indexing.indexing (range s e) i = Success v -> v = (s + i).
+      Indexing.Int.indexing (range s e) i = Success v -> v = (s + i).
     Proof. unfold range. intros. apply Impl.indexing with (1 := H). Qed.
 
-    Lemma completeness {F: Type} {f: Result.AssertionError F}: forall s e z, s <= z -> z < e -> exists i, Indexing.indexing (range s e) i = Success z.
+    Lemma completeness {F: Type} {f: Result.AssertionError F}: forall s e z, s <= z -> z < e -> exists i, Indexing.Int.indexing (range s e) i = Success z.
     Proof.
       intros. remember (z - s) as i.
       exists i.
       assert (0 <= i < Z.of_nat (Z.to_nat (e - s))) as Bounds_z by lia.
       rewrite <- length in Bounds_z.
-      destruct (Indexing.indexing (range s e) i) eqn:Eq.
+      destruct (Indexing.Int.indexing (range s e) i) eqn:Eq.
       - apply indexing in Eq. f_equal. lia.
-      - apply Indexing.failure_bounds in Eq. lia.
+      - apply Indexing.Int.failure_bounds in Eq. lia.
     Qed.
 
     Lemma range_sortedness {F: Type} {f: Result.AssertionError F}: forall s e i0 i1 z0 z1,
       (i0 <= i1)%Z ->
-      Indexing.indexing (range s e) i0 = Success z0 ->
-      Indexing.indexing (range s e) i1 = Success z1 ->
+      Indexing.Int.indexing (range s e) i0 = Success z0 ->
+      Indexing.Int.indexing (range s e) i1 = Success z1 ->
       (z0 <= z1)%Z.
     Proof. intros. apply indexing in H0. apply indexing in H1. lia. Qed.
   End Range.
