MECMAR/props/Incorrectness.v
@@ -4,10 +4,8 @@ From Warblre Require Import Tactics Specialize Focus Result Base Patterns Static
 Import Result.Notations.
 Import Semantics.
 
-Parameter a_: Character.
-Parameter char_eq_dec: Character -> Character -> bool.
-Axiom char_eq_refl: forall a, char_eq_dec a a = true.
-Definition a := Char (char_eq_dec a_) false.
+Parameter a: Character.
+Axiom char_eq_refl: forall a, (a =? a = true)%Chr.
 
 Module RegexNotations.
 
@@ -18,9 +16,11 @@ Module RegexNotations.
   Notation "'</' r '/>'"  := r (r custom regex at level 99).
   Notation "r1 '|' r2" := (Disjunction r1 r2) (in custom regex at level 99, right associativity).
   Notation "r1 '~' r2" := (Seq r1 r2) (in custom regex at level 50, right associativity).
-  Notation "'(|' n ':' r '|)'" := (Group (Z.of_nat n) r) (n constr at level 0, r at level 99, in custom regex at level 1).
+  Notation "'(|' n ':' r '|)'" := (Group n r) (n constr at level 0, r at level 99, in custom regex at level 1).
   Notation "'(' r ')'" := r (r at level 99, in custom regex at level 1).
   Notation "x" := x (in custom regex at level 0, x constr).
+
+  Coercion Char: Character >-> Regex.
 
   Example example_1: </ a | a ~ a | a /> = Disjunction a (Disjunction (Seq a a) a). reflexivity. Qed.
   Example example_2: </ (a | a) ~ a | a /> = Disjunction (Seq (Disjunction a a) a) a. reflexivity. Qed.
@@ -36,7 +36,7 @@ Module Incorrectness.
   Proof.
     exists </ (|0: a |) />. exists </ (|1: a |) />.
     exists (reg_exp 2).
-    exists (a_ :: nil). exists 0.
+    exists (a :: nil). exists 0.
     repeat( cbn || rewrite -> char_eq_refl || unfold Pos.to_nat ).
     easy.
   Qed.
