extraction/Extraction.v
@@ -8,12 +8,6 @@ From Coq Require extraction.ExtrOcamlString.
 From Coq Require extraction.ExtrOcamlNatInt.
 From Coq Require extraction.ExtrOcamlZInt.
 
-Extract Constant IdSet.t => "Interop.Ocaml_Set_Int.t".
-Extract Constant IdSet.empty => "Interop.Ocaml_Set_Int.empty".
-Extract Constant IdSet.add => "Interop.Ocaml_Set_Int.add".
-Extract Constant IdSet.union => "Interop.Ocaml_Set_Int.union".
-Extract Constant IdSet.fold => "Interop.Ocaml_Set_Int.fold".
-
 Extract Constant Character => "char".
 Extract Constant Character.eqb => "Char.equal".
 
